<<<<<<< HEAD
@prefix dct:  <http://purl.org/dc/terms/> .
@prefix gr:   <http://purl.org/goodrelations/v1#> .
@prefix mv:   <http://schema.mobivoc.org/#> .
@prefix owl:  <http://www.w3.org/2002/07/owl#> .
@prefix rdf:  <http://www.w3.org/1999/02/22-rdf-syntax-ns#> .
@prefix rdfs: <http://www.w3.org/2000/01/rdf-schema#> .
@prefix s:    <http://schema.org/> .
@prefix skos: <http://www.w3.org/2004/02/skos/core#> .
@prefix vs:   <http://www.w3.org/2003/06/sw-vocab-status/ns#> .
@prefix xsd:  <http://www.w3.org/2001/XMLSchema#> .

<https://material-digital.de/pmdco/hasProcessNodeIdentifier>
=======
@prefix :        <https://material-digital.de/pmdco/> .
@prefix DUL:     <http://www.loa-cnr.it/ontologies/DUL.owl#> .
@prefix dc:      <http://purl.org/dc/elements/1.1/> .
@prefix dct:     <http://purl.org/dc/terms/> .
@prefix dcterms: <http://purl.org/dc/terms/> .
@prefix dul:     <http://www.loa-cnr.it/ontologies/DUL.owl#> .
@prefix ex:      <http://example.org/> .
@prefix foaf:    <http://xmlns.com/foaf/spec/> .
@prefix geo:     <http://www.w3.org/2003/01/geo/wgs84_pos#> .
@prefix gr:      <http://purl.org/goodrelations/v1#> .
@prefix mv:      <http://schema.mobivoc.org/#> .
@prefix obda:    <https://w3id.org/obda/vocabulary#> .
@prefix om:      <http://www.wurvoc.org/vocabularies/om-1.8/> .
@prefix owl:     <http://www.w3.org/2002/07/owl#> .
@prefix prov:    <http://www.w3.org/ns/prov#> .
@prefix rami:    <https://w3id.org/i40/rami#> .
@prefix rdf:     <http://www.w3.org/1999/02/22-rdf-syntax-ns#> .
@prefix rdfs:    <http://www.w3.org/2000/01/rdf-schema#> .
@prefix s:       <http://schema.org/> .
@prefix skos:    <http://www.w3.org/2004/02/skos/core#> .
@prefix ssn:     <http://purl.oclc.org/NET/ssnx/ssn#> .
@prefix sto:     <https://w3id.org/i40/sto#> .
@prefix vann:    <http://purl.org/vocab/vann/> .
@prefix vcard:   <http://www.w3.org/2006/vcard/ns#> .
@prefix voaf:    <http://purl.org/vocommons/voaf#> .
@prefix void:    <http://rdfs.org/ns/void#> .
@prefix vs:      <http://www.w3.org/2003/06/sw-vocab-status/ns#> .
@prefix wd:      <http://www.wikidata.org/entity/> .
@prefix wdt:     <http://www.wikidata.org/prop/direct/> .
@prefix xml:     <http://www.w3.org/XML/1998/namespace> .
@prefix xsd:     <http://www.w3.org/2001/XMLSchema#> .

:hasProcessNodeIdentifier
>>>>>>> e19ea1c5ccd4723f06d43bbc270bbfc07d616d1c
        rdf:type            owl:DatatypeProperty ;
        rdfs:comment        "A string intended to uniquely identify a process node in a given scope, e.g. global scope: serial number, organization scope, asset management identifier."@en ;
        rdfs:label          "has process node identifier"@en ;
        rdfs:subPropertyOf  <https://material-digital.de/pmdco/hasProcessNodeCharacteristic> .

<https://material-digital.de/pmdco/hasProcessNodeCharacteristic>
        rdf:type      owl:DatatypeProperty ;
        rdfs:comment  "The point in time a process node was commissioned (e.g. the purchase date, first day of use), represented in IEEE 1003 'Seconds since Epoch'."@en ;
        rdfs:domain   <https://material-digital.de/pmdco/ProcessNode> ;
        rdfs:label    "has process node characteristic"@en ;
        rdfs:range    rdfs:Literal .

<https://material-digital.de/pmdco/ProcessNodeComponent>
        rdf:type    owl:Class ;
        rdfs:label  "Process Node Component"@en .

<https://material-digital.de/pmdco/HeaderField>
        rdf:type      owl:Class ;
        rdfs:comment  "A class bundling the semantics for a specific column in a table inside a (multidimensional) blob. Includes column number, pointer to concept, pointer to unit, and human readable description."@en ;
        rdfs:label    "Header Field"@en .

<https://material-digital.de/pmdco/suppliedObjectIdentifier>
        rdf:type            owl:DatatypeProperty ;
        rdfs:comment        "A human-generated identifier associated with a discernable, tangible or simulated entity"@en ;
        rdfs:domain         <https://material-digital.de/pmdco/Object> ;
        rdfs:label          "supplied object identifier"@en ;
        rdfs:range          xsd:string ;
        rdfs:subPropertyOf  <https://material-digital.de/pmdco/objectCharacteristics> .

<https://material-digital.de/pmdco/Object>
        rdf:type      owl:Class ;
        rdfs:comment  "A discernable, tangible or simulated entity that is processed in a process by a process node. An Object is composed of Voxels."@en ;
        rdfs:label    "Object"@en .

<https://material-digital.de/pmdco/objectCharacteristics>
        rdf:type    owl:DatatypeProperty ;
        rdfs:label  "has object characteristic"@en .

<https://material-digital.de/pmdco/hasNominalStartPosixTimestamp>
        rdf:type            owl:DatatypeProperty ;
        rdfs:comment        "The point in time a process node began to conduct a process, represented in IEEE 1003 'Seconds since Epoch'"@en ;
        rdfs:label          "has nominal start posix timestamp"@en ;
        rdfs:subPropertyOf  <https://material-digital.de/pmdco/hasNominalMetadataParameter> .

<https://material-digital.de/pmdco/hasNominalMetadataParameter>
        rdf:type            owl:DatatypeProperty ;
        rdfs:domain         <https://material-digital.de/pmdco/Process> ;
        rdfs:label          "has nominal metadata parameter"@en ;
        rdfs:range          rdfs:Literal ;
        rdfs:subPropertyOf  <https://material-digital.de/pmdco/hasNominalParameter> .

<https://material-digital.de/pmdco/hasTypeDescription>
        rdf:type            owl:DatatypeProperty ;
        rdfs:comment        "Description for Process Node's utility, e.g. \"Rear Vacuum Furnace Oil Quenching\""@en ;
        rdfs:domain         <https://material-digital.de/pmdco/ProcessNode> ;
        rdfs:label          "has type description"@en ;
        rdfs:range          xsd:string ;
        rdfs:subPropertyOf  <https://material-digital.de/pmdco/hasProcessNodeCharacteristic> .

<https://material-digital.de/pmdco/ProcessNode>
        rdf:type      owl:Class ;
        rdfs:comment  "A constituent that consumes and creates the objects in a process. The enabler of manufacture process steps, analysis process steps or simulation process steps. A process node realizes transformative processes and/or non-transformative processes."@en ;
        rdfs:label    "ProcessNode"@en .

<https://material-digital.de/pmdco/hasQuantitativeNominalParameter>
        rdf:type            owl:ObjectProperty ;
        rdfs:comment        "This property is used to describe a quantity value that was input of process."@en ;
        rdfs:domain         [ rdf:type     owl:Class ;
                              owl:unionOf  ( <https://material-digital.de/pmdco/Object> <https://material-digital.de/pmdco/Process> )
                            ] ;
        rdfs:label          "has quantitative nominal parameter"@en ;
        rdfs:range          [ rdf:type     owl:Class ;
                              owl:unionOf  ( <http://wikiba.se/ontology#QuantityValue> <https://material-digital.de/pmdco/HeaderField> )
                            ] ;
        rdfs:subPropertyOf  <https://material-digital.de/pmdco/hasQuantitativeParameter> .

<https://material-digital.de/pmdco/Process>
        rdf:type      owl:Class ;
        rdfs:comment  "A series of actions or operations conducing to an end\nIn PMD, a process is conducted via process nodes and has a discernable duration as part of a workflow. A process consumes objects and parameters. A process potentially generates new objects and measurements. A process is either a transformative process or a non-transformative process with respect to objects processed via a process node. There are primarily two types of distinguishable processes: manufacture process, analysis process. A process is a series of operations that are subordinate processes."@en ;
        rdfs:label    "Process"@en .

<http://wikiba.se/ontology#QuantityValue>
        rdf:type         owl:Class ;
        rdfs:comment     "Wikibase extended value representing quantity." ;
        rdfs:label       "QuantityValue" ;
        rdfs:subClassOf  <http://wikiba.se/ontology#Value> .

<https://material-digital.de/pmdco/hasQuantitativeParameter>
        rdf:type      owl:ObjectProperty ;
        rdfs:comment  "This property is used to relate values with units to process measurements and paramaeters."@en ;
        rdfs:domain   [ rdf:type     owl:Class ;
                        owl:unionOf  ( <https://material-digital.de/pmdco/Object> <https://material-digital.de/pmdco/Process> )
                      ] ;
        rdfs:label    "has quantitative parameter"@en ;
        rdfs:range    [ rdf:type     owl:Class ;
                        owl:unionOf  ( <http://wikiba.se/ontology#QuantityValue> <https://material-digital.de/pmdco/HeaderField> )
                      ] .

<https://material-digital.de/pmdco/DataResource>
        rdf:type      owl:Class ;
        rdfs:comment  "A data resource is file which contains parameters and measurements of a process."@en ;
        rdfs:label    "Data Resource"@en .

<https://material-digital.de/pmdco/SimulationNode>
        rdf:type         owl:Class ;
        rdfs:comment     "A process node that implements foo as well as consumes and creates simulation objects and parameters."@en ;
        rdfs:label       "Simulation Node"@en ;
        rdfs:subClassOf  <https://material-digital.de/pmdco/ProcessNode> .

<http://wikiba.se/ontology#quantityUnit>
        rdf:type      owl:ObjectProperty ;
        rdfs:comment  "Unit of measurement." ;
        rdfs:domain   <http://wikiba.se/ontology#QuantityValue> ;
        rdfs:label    "quantityUnit" ;
        rdfs:range    <http://wikiba.se/ontology#Item> .

<http://wikiba.se/ontology#Item>
        rdf:type  owl:Class .

<https://material-digital.de/pmdco/hasNominalPrimaryParameter>
        rdf:type            owl:DatatypeProperty ;
        rdfs:domain         <https://material-digital.de/pmdco/Process> ;
        rdfs:label          "has nominal primary parameter"@en ;
        rdfs:range          rdfs:Literal ;
        rdfs:subPropertyOf  <https://material-digital.de/pmdco/hasNominalParameter> .

<https://material-digital.de/pmdco/hasNominalParameter>
        rdf:type            owl:DatatypeProperty ;
        rdfs:comment        "This property is used to describe nominal parameters that are not associated to a quantity value."@en ;
        rdfs:domain         <https://material-digital.de/pmdco/Process> ;
        rdfs:label          "has nominal parameter"@en ;
        rdfs:range          rdfs:Literal ;
        rdfs:subPropertyOf  <https://material-digital.de/pmdco/hasParameter> .

<https://material-digital.de/pmdco/MicroscopicLevelMaterialStructure>
        rdf:type         owl:Class ;
        rdfs:comment     "A material structure on a single grain level"@en ;
        rdfs:label       "Microscopic Level Material Structure"@en ;
        rdfs:subClassOf  <https://material-digital.de/pmdco/MaterialStructure> .

<https://material-digital.de/pmdco/MaterialStructure>
        rdf:type      owl:Class ;
        rdfs:comment  "Structural and compositional information on a material within the regarded material level, includes 0,1,2,3 dimensional descriptions involves all material levels."@en ;
        rdfs:label    "Material Structure"@en .

<https://material-digital.de/pmdco/ManufactureNode>
        rdf:type         owl:Class ;
        rdfs:comment     "A process node that implements transformative processes as well as consumes and creates tangible objects and typically requires inputs\nIn general but not necessarily, a manufacture node includes intrinsic analysis nodes that create corresponding measurements with respect to the process implemented by the manufacture node."@en ;
        rdfs:label       "Manufacture Node"@en ;
        rdfs:subClassOf  <https://material-digital.de/pmdco/ProcessNode> .

<https://material-digital.de/pmdco/hasHeaderFieldSequenceNumber>
        rdf:type            owl:DatatypeProperty ;
        rdfs:comment        "A mandatory numbering representing the index of the columns in sequence"@en ;
        rdfs:domain         <https://material-digital.de/pmdco/HeaderField> ;
        rdfs:label          "has header field sequence number"@en ;
        rdfs:range          xsd:positiveInteger ;
        rdfs:subPropertyOf  <https://material-digital.de/pmdco/headerFieldCharacteristic> .

<https://material-digital.de/pmdco/headerFieldCharacteristic>
        rdf:type     owl:DatatypeProperty ;
        rdfs:domain  <https://material-digital.de/pmdco/HeaderField> ;
        rdfs:label   "has header field characteristic"@en ;
        rdfs:range   rdfs:Literal .

<https://material-digital.de/pmdco/hasNominalEndPosixTimestap>
        rdf:type            owl:DatatypeProperty ;
        rdfs:comment        "The point in time a process node finished to conduct a process, represented in IEEE 1003 'Seconds since Epoch'"@en ;
        rdfs:domain         <https://material-digital.de/pmdco/Process> ;
        rdfs:label          "has nominal end posix timestamp"@en ;
        rdfs:range          xsd:float ;
        rdfs:subPropertyOf  <https://material-digital.de/pmdco/hasNominalMetadataParameter> .

<https://material-digital.de/pmdco/Voxel>
        rdf:type      owl:Class ;
        rdfs:comment  "An element representing a value on a grid in three dimensional space.\nIn PMD, an infinitesimal part of an object which is made of a homogenuous material. Size depends on the observed material level. For now, geometrically, a cubus is assumed.\nMade of a material\nDifferent Voxels can have different material properties and material structure\nA (partial) logical object that describes (a part of) a physical object"@en ;
        rdfs:label    "Voxel"@en .

<https://material-digital.de/pmdco/NanoLevelMaterialStructure>
        rdf:type         owl:Class ;
        rdfs:comment     "A Material Structure that involves individual features within one single grain or phase like dislocations or precipitates."@en ;
        rdfs:label       "Nano Level Material Structure"@en ;
        rdfs:subClassOf  <https://material-digital.de/pmdco/MaterialStructure> .

<https://material-digital.de/pmdco/hasSecondaryMeasurement>
        rdf:type            owl:DatatypeProperty ;
        rdfs:domain         <https://material-digital.de/pmdco/Process> ;
        rdfs:label          "has secondary measurement"@en ;
        rdfs:range          rdfs:Literal ;
        rdfs:subPropertyOf  <https://material-digital.de/pmdco/hasMeasurement> .

<https://material-digital.de/pmdco/hasMeasurement>
        rdf:type            owl:DatatypeProperty ;
        rdfs:comment        "This property is used to describe parameters that are created by measurements of a process but that do not represent a quantity and are not associate to units."@en ;
        rdfs:domain         <https://material-digital.de/pmdco/Process> ;
        rdfs:label          "has measurement"@en ;
        rdfs:range          rdfs:Literal ;
        rdfs:subPropertyOf  <https://material-digital.de/pmdco/hasParameter> .

<https://material-digital.de/pmdco/hasSubordinateProcess>
        rdf:type      owl:ObjectProperty ;
        rdfs:comment  "This property is used to link a process to its subordinate processes."@en ;
        rdfs:domain   <https://material-digital.de/pmdco/Process> ;
        rdfs:label    "has subordinate process"@en ;
        rdfs:range    <https://material-digital.de/pmdco/Process> .

<https://material-digital.de/pmdco/hasDataResourceLocation>
        rdf:type            owl:DatatypeProperty ;
        rdfs:comment        "This property indicates that a file can be retrieved or downloaded from a specific address."@en ;
        rdfs:domain         <https://material-digital.de/pmdco/DataResource> ;
        rdfs:label          "has data resource location" ;
        rdfs:range          xsd:anyURI ;
        rdfs:subPropertyOf  <https://material-digital.de/pmdco/dataResourceCharacteristic> .

<https://material-digital.de/pmdco/dataResourceCharacteristic>
        rdf:type     owl:DatatypeProperty ;
        rdfs:domain  <https://material-digital.de/pmdco/DataResource> ;
        rdfs:label   "has data resource characteristic"@en ;
        rdfs:range   rdfs:Literal .

<https://material-digital.de/pmdco/MesoscopicLevelMaterialStructure>
        rdf:type         owl:Class ;
        rdfs:comment     "A material structure that covers multiple grains or phases of the material"@en ;
        rdfs:label       "Mesoscopic Level Material Structure"@en ;
        rdfs:subClassOf  <https://material-digital.de/pmdco/MaterialStructure> .

<https://material-digital.de/pmdco/hasParameter>
        rdf:type      owl:DatatypeProperty ;
        rdfs:comment  "This Property is used to describe the process parameters that are not associated to quantitative values."@en ;
        rdfs:domain   <https://material-digital.de/pmdco/Process> ;
        rdfs:label    "has parameter"@en ;
        rdfs:range    rdfs:Literal .

<https://material-digital.de/pmdco/hasDataResource>
        rdf:type      owl:ObjectProperty ;
        rdfs:comment  "This property is used to connect a Process to the Data Resource that describe the parameters and measurements produced during the process."@en ;
        rdfs:domain   <https://material-digital.de/pmdco/Process> ;
        rdfs:label    "has data resource"@en ;
        rdfs:range    <https://material-digital.de/pmdco/DataResource> .

<https://material-digital.de/pmdco/AnalysisProcess>
        rdf:type         owl:Class ;
        rdfs:comment     "A process that is driven by the primary intent to gain new measurements\nAn analysis process is either a transformative process or a non-transformative process."@en ;
        rdfs:label       "Analysis Process"@en ;
        rdfs:subClassOf  <https://material-digital.de/pmdco/Process> .

<https://material-digital.de/pmdco/>
        rdf:type  owl:Ontology .

<https://material-digital.de/pmdco/hasQuantitativeMetadataMeasurement>
        rdf:type            owl:ObjectProperty ;
        rdfs:domain         [ rdf:type     owl:Class ;
                              owl:unionOf  ( <https://material-digital.de/pmdco/Object> <https://material-digital.de/pmdco/Process> )
                            ] ;
        rdfs:label          "has quantitative metadata measurement"@en ;
        rdfs:range          [ rdf:type     owl:Class ;
                              owl:unionOf  ( <http://wikiba.se/ontology#QuantityValue> <https://material-digital.de/pmdco/HeaderField> )
                            ] ;
        rdfs:subPropertyOf  <https://material-digital.de/pmdco/hasQuantitativeMeasurement> .

<https://material-digital.de/pmdco/hasQuantitativeMeasurement>
        rdf:type            owl:ObjectProperty ;
        rdfs:comment        "This property is used to describe a quantity value that has been measured during the execution of a process."@en ;
        rdfs:domain         [ rdf:type     owl:Class ;
                              owl:unionOf  ( <https://material-digital.de/pmdco/Object> <https://material-digital.de/pmdco/Process> )
                            ] ;
        rdfs:label          "has quantitative measurement"@en ;
        rdfs:range          [ rdf:type     owl:Class ;
                              owl:unionOf  ( <http://wikiba.se/ontology#QuantityValue> <https://material-digital.de/pmdco/HeaderField> )
                            ] ;
        rdfs:subPropertyOf  <https://material-digital.de/pmdco/hasQuantitativeParameter> .

<https://material-digital.de/pmdco/hasStartingTime>
        rdf:type     owl:DatatypeProperty ;
        rdfs:domain  <https://material-digital.de/pmdco/Process> ;
        rdfs:label   "has starting time"@en ;
        rdfs:range   rdfs:Literal .

<https://material-digital.de/pmdco/hasInputObject>
        rdf:type      owl:ObjectProperty ;
        rdfs:comment  "This property is used to link the processes to their input objects"@en ;
        rdfs:domain   <https://material-digital.de/pmdco/Process> ;
        rdfs:label    "has input object"@en ;
        rdfs:range    <https://material-digital.de/pmdco/Object> .

<https://material-digital.de/pmdco/hasPmdUnit>
        rdf:type      owl:ObjectProperty ;
        rdfs:comment  "The association of a higher concept with a unit of measurement from Wikidata"@en ;
        rdfs:domain   [ rdf:type     owl:Class ;
                        owl:unionOf  ( <http://wikiba.se/ontology#QuantityValue> <https://material-digital.de/pmdco/HeaderField> )
                      ] ;
        rdfs:label    "has pmd quantity unit"@en ;
        rdfs:range    <https://material-digital.de/pmdco/PmdSiUnit> .

<https://material-digital.de/pmdco/PmdSiUnit>
        rdf:type      owl:Class ;
        rdfs:comment  "Equivalent to the definition found at https://www.wikidata.org/wiki/Q61610698. Instances of this class represent a tuple of prefix and SI unit"@en ;
        rdfs:label    "PmdSiUnit"@en .

<https://material-digital.de/pmdco/hasSequenceNumber>
        rdf:type            owl:DatatypeProperty ;
        rdfs:domain         <https://material-digital.de/pmdco/Process> ;
        rdfs:label          "has sequence number"@en ;
        rdfs:range          xsd:positiveInteger ;
        rdfs:subPropertyOf  <https://material-digital.de/pmdco/hasNominalMetadataParameter> .

<https://material-digital.de/pmdco/hasMaterialStructure>
        rdf:type      owl:ObjectProperty ;
        rdfs:comment  "This property is used to indicate which material structures a voxel has."@en ;
        rdfs:domain   <https://material-digital.de/pmdco/Voxel> ;
        rdfs:label    "has material structure"@en ;
        rdfs:range    <https://material-digital.de/pmdco/MaterialStructure> .

<https://material-digital.de/pmdco/hasAcquisitionDate>
        rdf:type            owl:DatatypeProperty ;
        rdfs:comment        "The point in time a process node was commissioned (e.g. the purchase date, first day of use), represented in IEEE 1003 'Seconds since Epoch'."@en ;
        rdfs:domain         <https://material-digital.de/pmdco/ProcessNode> ;
        rdfs:label          "has acquisition date"@en ;
        rdfs:range          xsd:positiveInteger ;
        rdfs:subPropertyOf  <https://material-digital.de/pmdco/hasProcessNodeCharacteristic> .

<https://material-digital.de/pmdco/hasQuantitativeNominalPrimaryParameter>
        rdf:type            owl:ObjectProperty ;
        rdfs:comment        "This property is used to describe a quantity value that is input of a process describing a primary process parameter."@en ;
        rdfs:domain         [ rdf:type     owl:Class ;
                              owl:unionOf  ( <https://material-digital.de/pmdco/Object> <https://material-digital.de/pmdco/Process> )
                            ] ;
        rdfs:label          "has quantitative nominal primary parameter"@en ;
        rdfs:range          [ rdf:type     owl:Class ;
                              owl:unionOf  ( <http://wikiba.se/ontology#QuantityValue> <https://material-digital.de/pmdco/HeaderField> )
                            ] ;
        rdfs:subPropertyOf  <https://material-digital.de/pmdco/hasQuantitativeNominalParameter> .

<https://material-digital.de/pmdco/execute>
        rdf:type            owl:ObjectProperty ;
        rdfs:comment        "This property represents which process node executes a process"@en ;
        rdfs:domain         <https://material-digital.de/pmdco/ProcessNode> ;
        rdfs:label          "execute"@en ;
        rdfs:range          <https://material-digital.de/pmdco/Process> ;
        rdfs:subPropertyOf  owl:topObjectProperty .

<https://material-digital.de/pmdco/NonTransformativeAnalysisProcess>
        rdf:type         owl:Class ;
        rdfs:comment     "An analysis process that is also a non-transformative process"@en ;
        rdfs:label       "Non Transformative Analysis Process"@en ;
        rdfs:subClassOf  <https://material-digital.de/pmdco/AnalysisProcess> .

<https://material-digital.de/pmdco/hasHeaderField>
        rdf:type      owl:ObjectProperty ;
        rdfs:comment  "A description for each header field included in the blob represented by the data resource"@en ;
        rdfs:domain   <https://material-digital.de/pmdco/DataResource> ;
        rdfs:label    "has header field"@en ;
        rdfs:range    <https://material-digital.de/pmdco/HeaderField> .

<https://material-digital.de/pmdco/isInitialProcessNode>
        rdf:type            owl:DatatypeProperty ;
        rdfs:comment        "This property is used to indicate the first process conducted by a process node in a series of processes conducted by the same process node."@en ;
        rdfs:domain         <https://material-digital.de/pmdco/Process> ;
        rdfs:label          "is initial process node"@en ;
        rdfs:range          xsd:boolean ;
        rdfs:subPropertyOf  <https://material-digital.de/pmdco/hasNominalMetadataParameter> .

<https://material-digital.de/pmdco/hasMetadataMeasurement>
        rdf:type            owl:DatatypeProperty ;
        rdfs:domain         <https://material-digital.de/pmdco/Process> ;
        rdfs:label          "has metadata measurement"@en ;
        rdfs:range          rdfs:Literal ;
        rdfs:subPropertyOf  <https://material-digital.de/pmdco/hasMeasurement> .

<https://material-digital.de/pmdco/hasPreviousProcess>
        rdf:type      owl:ObjectProperty ;
        rdfs:comment  "This property is used to indicate that which process was previously run."@en ;
        rdfs:domain   <https://material-digital.de/pmdco/Process> ;
        rdfs:label    "has previous process"@en ;
        rdfs:range    <https://material-digital.de/pmdco/Process> .

<https://material-digital.de/pmdco/hasModel>
        rdf:type            owl:DatatypeProperty ;
        rdfs:comment        "Process Node short description, e.g. \"Vacuum Furnace\""@en ;
        rdfs:domain         <https://material-digital.de/pmdco/ProcessNode> ;
        rdfs:label          "has model"@en ;
        rdfs:range          xsd:string ;
        rdfs:subPropertyOf  <https://material-digital.de/pmdco/hasProcessNodeCharacteristic> .

<https://material-digital.de/pmdco/hasGeneratedIdentifier>
        rdf:type            owl:DatatypeProperty ;
        rdfs:comment        "A machine-readable identifier that is intended to be unique in a given scope."@en ;
        rdfs:domain         [ rdf:type     owl:Class ;
                              owl:unionOf  ( <https://material-digital.de/pmdco/Object> <https://material-digital.de/pmdco/Process> <https://material-digital.de/pmdco/ProcessNode> )
                            ] ;
        rdfs:label          "has generated identifier"@en ;
        rdfs:range          xsd:string ;
        rdfs:subPropertyOf  <https://material-digital.de/pmdco/hasNominalMetadataParameter> .

<https://material-digital.de/pmdco/composedBy>
        rdf:type      owl:ObjectProperty ;
        rdfs:comment  "This property is used to describe which voxels and materials an object is composed of."@en ;
        rdfs:domain   <https://material-digital.de/pmdco/Object> ;
        rdfs:label    "composed by"@en ;
        rdfs:range    [ rdf:type     owl:Class ;
                        owl:unionOf  ( <https://material-digital.de/pmdco/Material> <https://material-digital.de/pmdco/Voxel> )
                      ] .

<https://material-digital.de/pmdco/Material>
        rdf:type      owl:Class ;
        rdfs:comment  "It is a substance or mixture of substances that constitutes an object.\nrepresented by the sum of material properties and material structure"@en ;
        rdfs:label    "Material"@en .

<https://material-digital.de/pmdco/isFinalProcessNode>
        rdf:type            owl:DatatypeProperty ;
        rdfs:comment        "This property is used to indicate the last process conducted by a process node in a series of processes conducted by the same process node."@en ;
        rdfs:domain         <https://material-digital.de/pmdco/Process> ;
        rdfs:label          "is final process node"@en ;
        rdfs:range          xsd:boolean ;
        rdfs:subPropertyOf  <https://material-digital.de/pmdco/hasNominalMetadataParameter> .

<https://material-digital.de/pmdco/hasQuantitativePrimaryDataSeriesMeasurement>
        rdf:type            owl:ObjectProperty ;
        rdfs:domain         <https://material-digital.de/pmdco/Process> ;
        rdfs:label          "has quantitative primary data series measurement"@en ;
        rdfs:range          <https://material-digital.de/pmdco/HeaderField> ;
        rdfs:subPropertyOf  <https://material-digital.de/pmdco/hasQuantitativePrimaryMetadata> .

<https://material-digital.de/pmdco/hasQuantitativePrimaryMetadata>
        rdf:type            owl:ObjectProperty ;
        rdfs:domain         [ rdf:type     owl:Class ;
                              owl:unionOf  ( <https://material-digital.de/pmdco/Object> <https://material-digital.de/pmdco/Process> )
                            ] ;
        rdfs:label          "has quantitative primary measurement"@en ;
        rdfs:range          [ rdf:type     owl:Class ;
                              owl:unionOf  ( <http://wikiba.se/ontology#QuantityValue> <https://material-digital.de/pmdco/HeaderField> )
                            ] ;
        rdfs:subPropertyOf  <https://material-digital.de/pmdco/hasQuantitativeMeasurement> .

<http://wikiba.se/ontology#Value>
        rdf:type  owl:Class .

<https://material-digital.de/pmdco/ManufactureProcess>
        rdf:type         owl:Class ;
        rdfs:comment     "A process that is driven by the primary intent to transform objects\nA manufacture process is always a transformative process."@en ;
        rdfs:label       "Manufacture Process"@en ;
        rdfs:subClassOf  <https://material-digital.de/pmdco/Process> .

<https://material-digital.de/pmdco/hasProcessNodeName>
        rdf:type            owl:DatatypeProperty ;
        rdfs:comment        "A human-generated identifier associated with a discernible, tangible or simulated entity intended to be unique in a given scope"@en ;
        rdfs:domain         <https://material-digital.de/pmdco/ProcessNode> ;
        rdfs:label          "has process node name"@en ;
        rdfs:range          xsd:string ;
        rdfs:subPropertyOf  <https://material-digital.de/pmdco/hasProcessNodeCharacteristic> .

<https://material-digital.de/pmdco/nominalProcessDuration>
        rdf:type            owl:ObjectProperty ;
        rdfs:domain         <https://material-digital.de/pmdco/Process> ;
        rdfs:label          "nominal process duration"@en ;
        rdfs:range          <http://wikiba.se/ontology#QuantityValue> ;
        rdfs:subPropertyOf  <https://material-digital.de/pmdco/hasQuantitativeNominalPrimaryParameter> .

<https://material-digital.de/pmdco/ContinuumLevelMaterialStructure>
        rdf:type         owl:Class ;
        rdfs:comment     "A material structure that is at the length level of the the entire geometry."@en ;
        rdfs:label       "Continuum Level Material Structure"@en ;
        rdfs:subClassOf  <https://material-digital.de/pmdco/MaterialStructure> .

<https://material-digital.de/pmdco/hasNominalSecondaryParameter>
        rdf:type            owl:DatatypeProperty ;
        rdfs:domain         <https://material-digital.de/pmdco/Process> ;
        rdfs:label          "has nominal secondary parameter"@en ;
        rdfs:range          rdfs:Literal ;
        rdfs:subPropertyOf  <https://material-digital.de/pmdco/hasNominalParameter> .

<https://material-digital.de/pmdco/AtomisticLevelMaterialStructure>
        rdf:type         owl:Class ;
        rdfs:comment     "It is a material length scale. Includes individual atoms and their spatial arrangement, information on the chemical elements, information on the lattice and crystal structure, 0-dimensional crystal defects"@en ;
        rdfs:label       "Atomistic Level Material Structure"@en ;
        rdfs:subClassOf  <https://material-digital.de/pmdco/MaterialStructure> .

<https://material-digital.de/pmdco/compose>
        rdf:type       owl:ObjectProperty ;
        rdfs:comment   "This property is used to describe which objects a voxel or a material contributes to compose."@en ;
        rdfs:domain    [ rdf:type     owl:Class ;
                         owl:unionOf  ( <https://material-digital.de/pmdco/Material> <https://material-digital.de/pmdco/Voxel> )
                       ] ;
        rdfs:label     "compose"@en ;
        rdfs:range     <https://material-digital.de/pmdco/Object> ;
        owl:inverseOf  <https://material-digital.de/pmdco/composedBy> .

<https://material-digital.de/pmdco/hasQuantitativeNominalSecondaryParameter>
        rdf:type            owl:ObjectProperty ;
        rdfs:comment        "This property is used to describe a quantity value that was input of process describing a secondary process parameter."@en ;
        rdfs:domain         [ rdf:type     owl:Class ;
                              owl:unionOf  ( <https://material-digital.de/pmdco/Object> <https://material-digital.de/pmdco/Process> )
                            ] ;
        rdfs:label          "has quantitative nominal secondary parameter"@en ;
        rdfs:range          [ rdf:type     owl:Class ;
                              owl:unionOf  ( <http://wikiba.se/ontology#QuantityValue> <https://material-digital.de/pmdco/HeaderField> )
                            ] ;
        rdfs:subPropertyOf  <https://material-digital.de/pmdco/hasQuantitativeNominalParameter> .

<https://material-digital.de/pmdco/TranformativeAnalysisProcess>
        rdf:type         owl:Class ;
        rdfs:comment     "An analysis process that is also a transformative process"@en ;
        rdfs:label       "Tranformative Analysis Process"@en ;
        rdfs:subClassOf  <https://material-digital.de/pmdco/AnalysisProcess> .

<https://material-digital.de/pmdco/hasQuantitativeNominalMetadataParameter>
        rdf:type            owl:ObjectProperty ;
        rdfs:comment        "This property is used to describe a quantity value that is input of a process describing a metadata process parameter."@en ;
        rdfs:domain         [ rdf:type     owl:Class ;
                              owl:unionOf  ( <https://material-digital.de/pmdco/Object> <https://material-digital.de/pmdco/Process> )
                            ] ;
        rdfs:label          "has quantitative nominal metadata parameter"@en ;
        rdfs:range          [ rdf:type     owl:Class ;
                              owl:unionOf  ( <http://wikiba.se/ontology#QuantityValue> <https://material-digital.de/pmdco/HeaderField> )
                            ] ;
        rdfs:subPropertyOf  <https://material-digital.de/pmdco/hasQuantitativeNominalParameter> .

<https://material-digital.de/pmdco/hasNextProcess>
        rdf:type      owl:ObjectProperty ;
        rdfs:comment  "This property is used to indicate the process that was run after the current process."@en ;
        rdfs:domain   <https://material-digital.de/pmdco/Process> ;
        rdfs:label    "has next process"@en ;
        rdfs:range    <https://material-digital.de/pmdco/Process> .

<https://material-digital.de/pmdco/hasUnitLabel>
        rdf:type      owl:DatatypeProperty ;
        rdfs:comment  "This property is used the enrich a unit with its common used label."@en ;
        rdfs:domain   <https://material-digital.de/pmdco/PmdSiUnit> ;
        rdfs:label    "has unit label"@en ;
        rdfs:range    rdfs:Literal .

<https://material-digital.de/pmdco/generatedObjectIdentifier>
        rdf:type            owl:DatatypeProperty ;
        rdfs:comment        "A machine-readable identifier associated with a discernable, tangible or simulated entity that is intended to be unique in a given scope. Examples for scope include: a database storing object data or a supply chain principal creating its own identifiers for the reports it generates"@en ;
        rdfs:domain         <https://material-digital.de/pmdco/Object> ;
        rdfs:label          "has generated object identifier"@en , "generated object identifier"@en ;
        rdfs:range          xsd:string ;
        rdfs:subPropertyOf  <https://material-digital.de/pmdco/objectCharacteristics> .

<https://material-digital.de/pmdco/hasOutputObject>
        rdf:type      owl:ObjectProperty ;
        rdfs:comment  "This property is used to link the processes to their output objects"@en ;
        rdfs:domain   <https://material-digital.de/pmdco/Process> ;
        rdfs:label    "has output object"@en ;
        rdfs:range    <https://material-digital.de/pmdco/Object> .

<https://material-digital.de/pmdco/hasProcessNodeComponent>
        rdf:type      owl:ObjectProperty ;
        rdfs:comment  "An object property associating a process node with its (potentially modular) components, e.g. the chambers of a heat treatment furnace."@en ;
        rdfs:domain   <https://material-digital.de/pmdco/ProcessNode> ;
        rdfs:label    "has process node component"@en ;
        rdfs:range    <https://material-digital.de/pmdco/ProcessNodeComponent> .

<https://material-digital.de/pmdco/hasProcessNodeType>
        rdf:type            owl:DatatypeProperty ;
        rdfs:comment        "Process Node typename, e.g. \"ProTherm500\""@en ;
        rdfs:domain         <https://material-digital.de/pmdco/ProcessNode> ;
        rdfs:label          "has process node type"@en ;
        rdfs:range          xsd:string ;
        rdfs:subPropertyOf  <https://material-digital.de/pmdco/hasProcessNodeCharacteristic> .

<http://wikiba.se/ontology#quantityAmount>
        rdf:type      owl:DatatypeProperty ;
        rdfs:comment  "Amount of quantity."@en ;
        rdfs:domain   <http://wikiba.se/ontology#QuantityValue> ;
        rdfs:label    "quantityAmount"@en ;
        rdfs:range    xsd:decimal .

<https://material-digital.de/pmdco/hasPrimaryMeasurement>
        rdf:type            owl:DatatypeProperty ;
        rdfs:domain         <https://material-digital.de/pmdco/Process> ;
        rdfs:label          "has primary measurement"@en ;
        rdfs:range          rdfs:Literal ;
        rdfs:subPropertyOf  <https://material-digital.de/pmdco/hasMeasurement> .

<https://material-digital.de/pmdco/hasHeaderFieldDescription>
        rdf:type            owl:DatatypeProperty ;
        rdfs:comment        "A data property representing an optional human-readable description of the header field's intent."@en ;
        rdfs:domain         <https://material-digital.de/pmdco/HeaderField> ;
        rdfs:label          "has header field description"@en ;
        rdfs:range          xsd:string ;
        rdfs:subPropertyOf  <https://material-digital.de/pmdco/headerFieldCharacteristic> .

<https://material-digital.de/pmdco/measuredProcessDuration>
        rdf:type            owl:ObjectProperty ;
        rdfs:domain         <https://material-digital.de/pmdco/Process> ;
        rdfs:label          "measured process duration"@en ;
        rdfs:range          <http://wikiba.se/ontology#QuantityValue> ;
        rdfs:subPropertyOf  <https://material-digital.de/pmdco/hasQuantitativePrimaryMetadata> .

<https://material-digital.de/pmdco/hasUcumCode>
        rdf:type            owl:DatatypeProperty ;
        rdfs:comment        "This property is used the enrich a unit with its common used label within the UCUM vocabulary"@en ;
        rdfs:domain         <https://material-digital.de/pmdco/PmdSiUnit> ;
        rdfs:label          "has ucum code"@en ;
        rdfs:range          rdfs:Literal ;
        rdfs:subPropertyOf  owl:topDataProperty .

<https://material-digital.de/pmdco/hasSuppliedIdentifier>
        rdf:type            owl:DatatypeProperty ;
        rdfs:comment        "A colloquial, human-generated, descriptive text qualifying the nature of a process instance used as an identifier that is not strictly intended to be unique, e.g. \"1050°C30 840°C10/ÖL\"."@en ;
        rdfs:domain         [ rdf:type     owl:Class ;
                              owl:unionOf  ( <https://material-digital.de/pmdco/Object> <https://material-digital.de/pmdco/Process> <https://material-digital.de/pmdco/ProcessNode> )
                            ] ;
        rdfs:label          "has supplied identifier"@en ;
        rdfs:range          xsd:string ;
        rdfs:subPropertyOf  <https://material-digital.de/pmdco/hasNominalMetadataParameter> .

<https://material-digital.de/pmdco/Component>
        rdf:type         owl:Class ;
        rdfs:comment     "An object that serves a specific technical application. Constituent part of a compound of parts that builds a technical application"@en ;
        rdfs:label       "Component"@en ;
        rdfs:subClassOf  <https://material-digital.de/pmdco/Object> .

<https://material-digital.de/pmdco/MaterialProperty>
        rdf:type      owl:Class ;
        rdfs:comment  "Physical property of a material"@en ;
        rdfs:label    "Material Property"@en .

<https://material-digital.de/pmdco/hasDataResourceSerialization>
        rdf:type            owl:DatatypeProperty ;
        rdfs:comment        ""@en ;
        rdfs:domain         <https://material-digital.de/pmdco/DataResource> ;
        rdfs:label          "has data resource serialization"@en ;
        rdfs:range          [ rdf:type   rdfs:Datatype ;
                              owl:oneOf  [ rdf:type   rdf:List ;
                                           rdf:first  "CBOR" ;
                                           rdf:rest   [ rdf:type   rdf:List ;
                                                        rdf:first  "JSON" ;
                                                        rdf:rest   ()
                                                      ]
                                         ]
                            ] ;
        rdfs:subPropertyOf  <https://material-digital.de/pmdco/dataResourceCharacteristic> .

<https://material-digital.de/pmdco/hasCollectionInterfaceHint>
        rdf:type            owl:DatatypeProperty ;
        rdfs:comment        "A label in support of identifying a network interface and/or address used by a process node to provide primary data stored in ontologies"@en ;
        rdfs:domain         <https://material-digital.de/pmdco/ProcessNode> ;
        rdfs:label          "has collection interface hint"@en ;
        rdfs:range          xsd:string ;
        rdfs:subPropertyOf  <https://material-digital.de/pmdco/hasProcessNodeCharacteristic> .

<https://material-digital.de/pmdco/hasProcessNodeVersion>
        rdf:type            owl:DatatypeProperty ;
        rdfs:comment        "Process Node Version Number, e.g. \"2.24\""@en ;
        rdfs:domain         <https://material-digital.de/pmdco/ProcessNode> ;
        rdfs:label          "has process node version"@en ;
        rdfs:range          xsd:string ;
        rdfs:subPropertyOf  <https://material-digital.de/pmdco/hasProcessNodeCharacteristic> .

<https://material-digital.de/pmdco/hasQuantitativeSecondaryMeasurement>
        rdf:type            owl:ObjectProperty ;
        rdfs:domain         [ rdf:type     owl:Class ;
                              owl:unionOf  ( <https://material-digital.de/pmdco/Object> <https://material-digital.de/pmdco/Process> )
                            ] ;
        rdfs:label          "has quantitative secondary measurement"@en ;
        rdfs:range          [ rdf:type     owl:Class ;
                              owl:unionOf  ( <http://wikiba.se/ontology#QuantityValue> <https://material-digital.de/pmdco/HeaderField> )
                            ] ;
        rdfs:subPropertyOf  <https://material-digital.de/pmdco/hasQuantitativeMeasurement> .
