@prefix :      <https://w3id.org/i40/rami#> .
@prefix obda:  <https://w3id.org/obda/vocabulary#> .
@prefix void:  <http://rdfs.org/ns/void#> .
@prefix owl:   <http://www.w3.org/2002/07/owl#> .
@prefix xsd:   <http://www.w3.org/2001/XMLSchema#> .
@prefix skos:  <http://www.w3.org/2004/02/skos/core#> .
@prefix rdfs:  <http://www.w3.org/2000/01/rdf-schema#> .
@prefix vcard: <http://www.w3.org/2006/vcard/ns#> .
@prefix ssn:   <http://purl.oclc.org/NET/ssnx/ssn#> .
@prefix sto:   <https://w3id.org/i40/sto#> .
@prefix geo:   <http://www.w3.org/2003/01/geo/wgs84_pos#> .
@prefix rdf:   <http://www.w3.org/1999/02/22-rdf-syntax-ns#> .
@prefix xml:   <http://www.w3.org/XML/1998/namespace> .
@prefix dcterms: <http://purl.org/dc/terms/> .
@prefix DUL:   <http://www.loa-cnr.it/ontologies/DUL.owl#> .
@prefix dul:   <http://www.loa-cnr.it/ontologies/DUL.owl#> .
@prefix vann:  <http://purl.org/vocab/vann/> .
@prefix prov:  <http://www.w3.org/ns/prov#> .
@prefix om:    <http://www.wurvoc.org/vocabularies/om-1.8/> .
@prefix foaf:  <http://xmlns.com/foaf/spec/> .
@prefix rami:  <https://w3id.org/i40/rami#> .
@prefix dc:    <http://purl.org/dc/elements/1.1/> .

rami:SensorMeasurementData
        a             owl:Class ;
        rdfs:comment  "Data measured by a sensor"@en ;
        rdfs:label    "Sensor Data"@en .

rami:subModelID  a          owl:FunctionalProperty , owl:DatatypeProperty ;
        rdfs:comment        "Unique Identification for a Submodel"@en ;
        rdfs:domain         rami:Submodel ;
        rdfs:label          "sub Model Id"@en ;
        rdfs:range          xsd:string ;
        rdfs:subPropertyOf  dcterms:identifier .

rami:Submodel  a      owl:Class ;
        rdfs:comment  "Describe the different types of Data related to the I4.0 Asset"@en ;
        rdfs:label    "Submodel"@en .

dcterms:identifier  a       owl:DatatypeProperty , owl:AnnotationProperty ;
        rdfs:range          rdfs:Literal ;
        rdfs:subPropertyOf  dc:identifier .

skos:note  a    owl:AnnotationProperty .

dc:publisher  a  owl:AnnotationProperty .

rami:Value  a         owl:Class ;
        rdfs:comment  "Current value that can be specified through an instanced submodel (for \ninstance in station 2) or through the asset, for example."@en ;
        rdfs:label    "Value"@en .

rami:contributes  a      owl:ObjectProperty ;
        rdfs:domain      rami:Submodel ;
        rdfs:range       prov:Agent ;
        skos:definition  "Agent(Person or Software) that contributes to the Entity/Object related data. It correspond to the Contributor concept of OMM"@en ;
        skos:prefLabel   "has Type Description"@en .

prov:Agent  a   owl:Class .

skos:definition  a  owl:AnnotationProperty .

skos:prefLabel  a  owl:AnnotationProperty .

rami:I4.0Component1  a          rami:I4.0Component , owl:NamedIndividual ;
        rdfs:label              "I4.0 Component 2"@en ;
        rami:containsAS         rami:AdminShell2 ;
        rami:hasI40ComponentId  "I40C112" .

rami:I4.0Component  a        owl:Class ;
        rdfs:comment         "Globally uniquely identifiable participant with communication capability consisting of administration shell and asset within an I4.0 system. \nSource: Industrie 4.0 – Begriffe/Terms, VDI Statusreport Industrie 4.0 (April 2017)"@en ;
        rdfs:isDefinedBy     "https://www.plattform-i40.de/I40/Navigation/EN/Service/Glossary/glossary.html" ;
        rdfs:label           "I4.0Component"@en ;
        owl:equivalentClass  [ a                            owl:Restriction ;
                               owl:minQualifiedCardinality  1 ;
                               owl:onClass                  rami:AdminShell ;
                               owl:onProperty               rami:containsAS
                             ] .

rami:containsAS  a    owl:ObjectProperty ;
        rdfs:comment  "Points the I4.0 Component to the Administration Shell"@en ;
        rdfs:domain   rami:I4.0Component ;
        rdfs:label    "contains Admin Shell"@en ;
        rdfs:range    rami:AdminShell .

rami:AdminShell2  a           owl:NamedIndividual , rami:AdminShell ;
        rdfs:label            "Admin Shell 2"@en ;
        rami:hasAdminShellId  "AAS112" ;
        rami:hasSubmodel      rami:EnergyEfficiency2 .

rami:hasI40ComponentId
        a                   owl:FunctionalProperty , owl:DatatypeProperty ;
        rdfs:comment        "Unique Identification of the Industry 4.0 component."@en ;
        rdfs:domain         rami:I4.0Component ;
        rdfs:label          "has I40 Component Id"@en ;
        rdfs:range          xsd:string ;
        rdfs:subPropertyOf  dcterms:identifier .

dc:coverage  a  owl:AnnotationProperty .

rami:Business  a  owl:NamedIndividual .

rami:AdminShell  a       owl:Class ;
        rdfs:label       "Admin Shell"@en ;
        dc:source        "This definition comprises material from RAMI4.0."@en ;
        skos:altLabel    "Asset Administration Shell"@en , "Administration Shell"@en ;
        skos:definition  "Describes the Administration Shell for Assets, Products, Components, e.g. Machines"@en ;
        skos:prefLabel   "Verwaltungsschale"@de .

rami:TechnicalData1  a  owl:NamedIndividual ;
        rdfs:label    "Technical Data 1"@en ;
        rami:display  "Seven-segment display"@en .

rami:display  a  owl:AnnotationProperty .

skos:example  a  owl:AnnotationProperty .

rami:usesStandard  a  owl:ObjectProperty ;
        rdfs:comment  "Points to the standards describing the functions attached to the asset via the administration shell"@en ;
        rdfs:label    "uses Standard"@en ;
        rdfs:range    sto:Standard .

sto:Standard  a           owl:Class ;
        rdfs:isDefinedBy  <https://w3id.org/i40/sto/#Standard> ;
        skos:definition   "Standards that are used to describe the actual I4.0 Asset. Defined in the STO ontology"@en ;
        skos:prefLabel    "Standard"@en .

rami:Structure  a        owl:Class ;
        rdfs:subClassOf  rami:Submodel .

rami:BrakingResistanceMs
        a                     owl:NamedIndividual , om:Measure ;
        om:hasNumericalValue  "60.0"^^xsd:float ;
        om:hasUnit            om:ohm .

om:Measure  a   owl:Class .

om:hasNumericalValue  a  owl:DatatypeProperty , owl:AnnotationProperty ;
        rdfs:domain  om:Measure ;
        rdfs:label   "has numerical value"@en .

om:hasUnit  a        owl:ObjectProperty ;
        rdfs:domain  om:Measure ;
        rdfs:label   "has unit"@en ;
        rdfs:range   om:Unit .

om:ohm  a       owl:NamedIndividual .

rami:hasSemanticExpression
        a             owl:ObjectProperty ;
        rdfs:comment  "Points to the Expression Semantic of the Submodels"@en ;
        rdfs:domain   rami:Submodel ;
        rdfs:label    "has Semantic Expression"@en ;
        rdfs:range    rami:ExpressionSemantic .

rami:ExpressionSemantic
        a                    owl:Class ;
        rdfs:comment         "Specifies which role the property plays in an interaction, i.e. which \nexpression the provider of the property intends. \nValid values are: Requirement (for requests that are to be confirmed or rejected) Confirmations (for responses to requests that describe the capability of an asset) Measurement (if a measured or actual value is provided)"@en ;
        rdfs:isDefinedBy     "https://www.zvei.org/fileadmin/user_upload/Presse_und_Medien/Publikationen/2017/April/Asset_Administration_Shell/ZVEI_WP_Verwaltungschale_Englisch_Download_03.04.17.pdf" ;
        rdfs:label           "Expression Semantic"@en , "Ausprägungsaussage"@de ;
        owl:equivalentClass  [ a          owl:Class ;
                               owl:oneOf  ( rami:Confirmation rami:Measurement rami:Requirement )
                             ] .

rami:Reference  a  owl:Class .

rami:Function  a      owl:NamedIndividual , rami:View ;
        rdfs:comment  "Makes statements on the function pursuant to IEC 81346 and on the function of the asset components.\nIncludes skills such as interpretation (?), commissioning, calculation (?) or diagnosis functions of the asset.\nExamples: current imbalance detection ability"@en ;
        rdfs:label    "Function"@en .

rami:View  a                 owl:Class ;
        rdfs:comment         "Different views associated to the Administration Shell via the Submodels"@en ;
        rdfs:isDefinedBy     "https://www.plattform-i40.de/I40/Redaktion/DE/Downloads/Publikation/hm-2018-trilaterale-coop.html"@de ;
        rdfs:label           "View" , "Sicht"@de ;
        owl:equivalentClass  [ a          owl:Class ;
                               owl:oneOf  ( rami:BusinessView rami:Construction rami:Function rami:Location rami:Performance )
                             ] .

dcterms:hasVersion  a  owl:AnnotationProperty .

skos:narrower  a  owl:AnnotationProperty .

rami:energyEfficiencyValue
        a             owl:ObjectProperty ;
        rdfs:comment  "Points to the value of the Energy Efficiency comsuption."@en ;
        rdfs:domain   rami:EnergyEfficiency ;
        rdfs:label    "energy Efficiency Value"@en ;
        rdfs:range    om:Measure .

rami:EnergyEfficiency
        a                owl:Class ;
        rdfs:subClassOf  rami:Submodel .

dc:identifier  a  owl:AnnotationProperty .

om:Unit  a      owl:Class .

dc:language  a  owl:AnnotationProperty .

rami:hasAssetId  a          owl:FunctionalProperty , owl:DatatypeProperty ;
        rdfs:comment        "Unique identification for the Asset."@en ;
        rdfs:domain         rami:Asset ;
        rdfs:label          "has Asset Id"@en ;
        rdfs:range          xsd:string ;
        rdfs:subPropertyOf  dcterms:identifier .

rami:Asset  a            owl:Class , owl:NamedIndividual ;
        skos:altLabel    "Entität"@de , "Entity"@en , "Object"@en ;
        skos:definition  "Eindeutig identifizierbarer Gegenstand, der aufgrund seiner Bedeutung in der Informationswelt verwaltet wird"@de , "Clearly identifiable asset for the Administration Shell"@en ;
        skos:note        "Objects may be known in the form of a type or of an instance. An object in the planning phase is known as a type"@en ;
        skos:prefLabel   "Asset"@en .

rami:Requirement  a   owl:NamedIndividual , rami:ExpressionSemantic ;
        rdfs:comment  "For requests that are to be confirmed or rejected"@en ;
        rdfs:label    "Requirement"@en .

rami:hasData  a          owl:ObjectProperty ;
        rdfs:domain      rami:AdminShell ;
        rdfs:range       rami:Submodel ;
        skos:definition  "Connects the AdminShell with the different types of Data for the Object/Entity"@en ;
        skos:prefLabel   "has Data"@en .

rami:Construction  a  owl:NamedIndividual , rami:View ;
        rdfs:comment  "Applies to the constructive deployment of the asset for selection, design of building structure or assemblies ...\nContains a structure classification system pursuant to IEC 81346.\nApplies to properties in respect of:\n1) physical dimensions and regarding start, processing and output values of the component.\n2) modular view of subcomponents or a asset structure and 3) inputs and outputs of different signal types."@en ;
        rdfs:label    "Construction"@en .

rami:LifeCycleDimension
        a                    owl:Class ;
        rdfs:label           "RAMI Life Cycle Dimension"@en ;
        rdfs:seeAlso         "http://www.zvei.org/en/subjects/Industry-40/Pages/The-Reference-Architectural-Model-RAMI-40-and-the-Industrie-40-Component.aspx" ;
        rdfs:seeAlso         <http://www.zvei.org/en/subjects/Industry-40/Pages/The-Reference-Architectural-Model-RAMI-40-and-the-Industrie-40-Component.aspx> ;
        rdfs:subClassOf      rami:Dimension ;
        owl:equivalentClass  [ a          owl:Class ;
                               owl:oneOf  ( rami:Instance rami:Type )
                             ] ;
        skos:definition      "It describes the different Life Cycle and Value Stream layers for the RAMI model according to the IEC 62890 Standard."@en ;
        skos:prefLabel       "RAMI Life Cycle Dimension"@en , "RAMI Layer"@en .

rami:Dimension  a     owl:Class ;
        rdfs:comment  "Abstract class to describe the three different dimensions of RAMI4.0"@en ;
        rdfs:label    "Dimension"@en .

rami:Instance  a  owl:NamedIndividual , rami:LifeCycleDimension .

rami:Type  a        owl:NamedIndividual , rami:LifeCycleDimension ;
        rdfs:label  "Type"@en .

rami:MeasureEnergyEfficiency1
        a                     owl:NamedIndividual , om:Measure ;
        rdfs:comment          "Measuring the Energy Efficiency for I4.0 component 1 in kilowattHour."@en ;
        rdfs:label            "Measure Energy Efficiency 1"@en ;
        owl:sameAs            rami:MeasureEnergyEfficiency2 ;
        om:hasNumericalValue  "17.3"^^xsd:float ;
        om:hasUnit            om:kilowattHour .

rami:MeasureEnergyEfficiency2
        a                     owl:NamedIndividual , om:Measure ;
        rdfs:comment          "Measuring the Energy Efficiency for I4.0 component 2 in Kilojoule."@en ;
        rdfs:label            "Measure Energy Efficiency 2"@en ;
        om:hasNumericalValue  "62280.0"^^xsd:float ;
        om:hasUnit            om:kilojoule .

om:kilowattHour  a  owl:NamedIndividual .

dul:isPartOf  a           owl:ObjectProperty , owl:TransitiveProperty ;
        rdfs:comment      "A relation between any entities, in this case, the Asset can be part of other Asset(s)." ;
        rdfs:domain       rami:Asset ;
        rdfs:isDefinedBy  <http://www.ontologydesignpatterns.org/ont/dul/DUL.owl> ;
        rdfs:label        "is Part Of"@en ;
        rdfs:range        rami:Asset .

rami:Platform  a  owl:Class .

rami:MESConnection  a    owl:Class ;
        rdfs:subClassOf  rami:Submodel .

skos:altLabel  a  owl:AnnotationProperty .

rami:maxOutputFrequencyMs
        a                     owl:NamedIndividual , om:Measure ;
        om:hasNumericalValue  "1.0"^^xsd:float ;
        om:hasUnit            om:hertz .

om:hertz  a     owl:NamedIndividual .

dc:subject  a   owl:AnnotationProperty .

rami:Station  a          owl:NamedIndividual , rami:HierarchyLevelDimension ;
        skos:definition  "Station hierarchy level of RAMI 4.0"@en ;
        skos:prefLabel   "Station"@en .

rami:HierarchyLevelDimension
        a                    owl:Class ;
        rdfs:seeAlso         <http://www.zvei.org/en/subjects/Industry-40/Pages/The-Reference-Architectural-Model-RAMI-40-and-the-Industrie-40-Component.aspx> ;
        rdfs:subClassOf      rami:Dimension ;
        owl:equivalentClass  [ a          owl:Class ;
                               owl:oneOf  ( rami:ConnectedWorld rami:ControlDevice rami:Enterprise rami:FieldDevice rami:Product rami:Station rami:WorkCenter )
                             ] ;
        skos:definition      "It describes the functional classification of various circumstances within Industrie 4.0. For classification within a factory, this axis of the reference architecture(layers) follows the IEC 62264 Standard."@en ;
        skos:prefLabel       "RAMI Hierarchy Level Dimension"@en .

rami:isDescribedWith  a  owl:DatatypeProperty , owl:ObjectProperty ;
        rdfs:domain      rami:AdminShell ;
        rdfs:range       sto:Standard ;
        skos:definition  "Points to the Standard used to describe a given object"@en ;
        skos:prefLabel   "Is Described With"@en .

rami:WorkCenter  a       owl:NamedIndividual , rami:HierarchyLevelDimension ;
        skos:definition  "Work Center hierarchy level of RAMI 4.0"@en ;
        skos:prefLabel   "Work Center"@en .

rami:hasManifest  a  owl:ObjectProperty ;
        rdfs:domain  rami:AdminShell ;
        rdfs:label   "has Manifest"@en ;
        rdfs:range   rami:Manifest .

rami:Manifest  a    owl:Class ;
        rdfs:label  "Manifest"@en .

rami:   a                              owl:Ontology ;
        rdfs:isDefinedBy               rami: ;
        vann:preferredNamespacePrefix  "rami" ;
        vann:preferredNamespaceUri     "https://w3id.org/i40/rami#" ;
        void:vocabulary                xsd: , foaf: , rdfs: , xml: , skos: , rdf: , dc: ;
        owl:versionInfo                "0.3" ;
        skos:definition                "An Ontology to represents the Reference Architecture Model for Industry 4.0 (RAMI), including the concept of the Administration Shell I4.0 Component."@en ;
        skos:prefLabel                 "rami"@en .

rami:creationDate  a     owl:DatatypeProperty ;
        rdfs:domain      rami:Submodel ;
        rdfs:range       xsd:dateTime ;
        skos:definition  "Date when an Agent(Person or Software) creates to the Entity/Object related data. It correspond to the Creator concept of OMM"@en ;
        skos:prefLabel   "has Creator"@en .

rami:Product  a          owl:NamedIndividual , rami:HierarchyLevelDimension ;
        skos:definition  "Product hierarchy level of RAMI 4.0"@en ;
        skos:prefLabel   "Product"@en .

rami:Integration  a  owl:NamedIndividual .

prov:wasGeneratedBy  a   owl:ObjectProperty ;
        rdfs:domain      rami:Submodel ;
        rdfs:range       prov:Agent ;
        skos:definition  "Agent (Person or Software) that generates the Asset related data. It correspond to the Creator concept of OMM"@en ;
        skos:prefLabel   "was Generated By"@en .

rami:Order  a            owl:Class ;
        skos:definition  "Each order for manufacturing runs through a life cycle and its specifics necessarily have an impact on the production facility during performance of the order"@en ;
        skos:prefLabel   "Order"@en .

dc:relation  a  owl:AnnotationProperty .

dc:creator  a   owl:AnnotationProperty .

skos:hiddenLabel  a  owl:AnnotationProperty .

dc:format  a    owl:AnnotationProperty .

rami:ConnectedWorld  a   owl:NamedIndividual , rami:HierarchyLevelDimension ;
        skos:definition  "Connected World hierarchy level of RAMI 4.0. Group of Factories, and the collaboration with external engineering firms, component suppliers and customers"@en ;
        skos:prefLabel   "Connected World"@en .

rami:ControlDevice  a    owl:NamedIndividual , rami:HierarchyLevelDimension ;
        skos:definition  "Control Device hierarchy level of RAMI 4.0"@en ;
        skos:prefLabel   "Control Device"@en .

rami:Enterprise  a       owl:NamedIndividual , rami:HierarchyLevelDimension ;
        skos:definition  "Enterprise hierarchy level of RAMI 4.0"@en ;
        skos:prefLabel   "Enterprise"@en .

rami:FieldDevice  a      owl:NamedIndividual , rami:HierarchyLevelDimension ;
        skos:definition  "Field Device hierarchy level of RAMI 4.0"@en ;
        skos:prefLabel   "Field Device"@en .

rami:CumulativeEnergyConsumption
        a       owl:Class .

rami:inAccordanceWith
        a             owl:ObjectProperty ;
        rdfs:comment  "The Submodel is in accordance with a given standard specified in the STO ontology"@en ;
        rdfs:domain   rami:Submodel ;
        rdfs:label    "in Accordance With"@en ;
        rdfs:range    sto:Standard .

rami:SensorMeasurement
        a                owl:Class ;
        rdfs:subClassOf  rami:Submodel .

rami:I4.0Component2  a          rami:I4.0Component , owl:NamedIndividual ;
        rdfs:label              "I4.0 Component 1"@en ;
        rami:containsAS         rami:AdminShell1 ;
        rami:hasI40ComponentId  "I40C111" .

rami:AdminShell1  a           owl:NamedIndividual , rami:AdminShell ;
        rdfs:label            "Admin Shell 1"@en ;
        rami:hasAdminShellId  "AAS111" ;
        rami:hasSubmodel      rami:EnergyEfficiency1 .

rami:isConnectedTo  a  owl:ObjectProperty ;
        rdfs:comment  "Connects the Admin Shell with the different RAMI4.0 Dimensions"@en ;
        rdfs:domain   rami:AdminShell ;
        rdfs:label    "is Connected To"@en ;
        rdfs:range    rami:Dimension .

rami:Functional  a  owl:NamedIndividual .

dc:source  a    owl:AnnotationProperty .

rami:AdminShellMotor  a  owl:NamedIndividual , rami:AdminShell ;
        rdfs:label      "Admin Shell Motor"@en ;
        rami:describes  rami:AssetMotorControl .

rami:describes  a     owl:ObjectProperty ;
        rdfs:comment  "Connect the Asset with the Administration Shell"@en ;
        rdfs:domain   rami:AdminShell ;
        rdfs:label    "describes"@en ;
        rdfs:range    rami:Asset .

rami:AssetMotorControl
        a                owl:NamedIndividual , rami:Asset ;
        rdfs:label       "Motor control"@en ;
        rami:hasAssetId  "1501325" .

dc:description  a  owl:AnnotationProperty .

rami:Asset1  a           owl:NamedIndividual , rami:Asset ;
        rdfs:label       "Asset 1"@en ;
        rami:hasAssetId  "AS711" .

rami:Communication  a  owl:NamedIndividual .

rami:Machine  a          owl:Class ;
        rdfs:subClassOf  rami:Asset ;
        skos:definition  "A machine is ordered, designed, commissioned, operated, serviced, converted and recycled."@en ;
        skos:prefLabel   "Machine"@en .

om:kilojoule  a  owl:NamedIndividual .

ssn:Sensor  a   owl:Class .

geo:lat  a            owl:DatatypeProperty ;
        rdfs:comment  "The WGS84 altitude of a SpatialThing (decimal meters above the local reference ellipsoid)."@en ;
        rdfs:domain   rami:Machine ;
        rdfs:label    "lat"@en ;
        rdfs:range    xsd:decimal .

rami:recordedTime  a    owl:DatatypeProperty ;
        rdfs:comment    "Recorded Time for a Machine"@en ;
        rdfs:domain     rami:Machine ;
        rdfs:range      xsd:dateTime ;
        skos:prefLabel  "recorded Time"@en .

rami:hasAdminShellId  a     owl:FunctionalProperty , owl:DatatypeProperty ;
        rdfs:domain         rami:AdminShell ;
        rdfs:range          xsd:string ;
        rdfs:subPropertyOf  dcterms:identifier ;
        skos:definition     "Unique Identification of the Administration Shell"@en ;
        skos:prefLabel      "has AdminShell Id"@en .

rami:hasSubmodel  a   owl:ObjectProperty ;
        rdfs:comment  "Points to the Admin Shell to the Submodels that describe the Admin Shell of a given Asset"@en ;
        rdfs:domain   rami:AdminShell ;
        rdfs:label    "has Submodel"@en ;
        rdfs:range    rami:Submodel .

rami:EnergyEfficiency1
        a                           owl:NamedIndividual , rami:EnergyEfficiency ;
        rdfs:label                  "Energy Efficiency 1 Submodel"@en ;
        skos:definition             "Integrated electrical consumption over time."@en ;
        skos:prefLabel              "Electrical consumption cumulative energy"@en ;
        rami:energyEfficiencyValue  rami:MeasureEnergyEfficiency1 ;
        rami:hasSemanticExpression  rami:Measurement ;
        rami:hasView                rami:Performance ;
        rami:subModelID             "AAB012" .

rami:BusinessView  a  owl:NamedIndividual , rami:View ;
        rdfs:label  "Business"@en , "Allows judging on the business suitability and performance of an asset.\nExamples: Manufacturer name, prices, terms of delivery, order codes.”"@en .

rami:Location  a      owl:NamedIndividual , rami:View ;
        rdfs:comment  "Describes the capabilities of the asset regarding environmental conditions and positions of the asset.\nDescribes the relationships capabilities of the asset or its parts or inputs and outputs with the linked assets.\nExamples: Degree of protection, working temperature, EMC characteristics, rated voltage, rated ultimate  \nshort-circuit breaking capacity."@en ;
        rdfs:label    "Location"@en .

rami:Performance  a   owl:NamedIndividual , rami:View ;
        rdfs:comment  "Describes performance and behavioural characteristics. Examples: To allow a performance assessment and virtual commissioning of an overall system. Example: instantaneous short-circuit current setting"@en ;
        rdfs:label    "Performance"@en .

rami:description  a      owl:DatatypeProperty ;
        rdfs:domain      rami:Asset ;
        rdfs:range       xsd:string ;
        skos:definition  "Description of the Object/Entity"@en ;
        skos:prefLabel   "has Description"@en .

rami:Measurement  a   owl:NamedIndividual , rami:ExpressionSemantic ;
        rdfs:comment  "If a measured or actual value is provided"@en ;
        rdfs:label    "Measurement"@en .

rami:hasView  a       owl:ObjectProperty ;
        rdfs:comment  "Points to the differents views associated to the Administration Shell via the Submodels."@en ;
        rdfs:domain   rami:Submodel ;
        rdfs:label    "has View"@en ;
        rdfs:range    rami:View .

rami:logs  a            owl:DatatypeProperty ;
        rdfs:range      xsd:string ;
        skos:prefLabel  "logs"@en .

ssn:SensorOutput  a          owl:Class ;
        owl:equivalentClass  rami:SensorMeasurementData .

dc:contributor  a  owl:AnnotationProperty .

rami:hasRAMILifeCycleLayer
        a                owl:ObjectProperty ;
        skos:definition  "Connects the concepts with the correspondent layer in the RAMI Hierarchy Levels"@en ;
        skos:prefLabel   "has RAMI Life Cycle Layer" .

rami:receivedAtTime  a   owl:DatatypeProperty ;
        rdfs:domain      rami:AdminShell ;
        rdfs:range       xsd:dateTime ;
        skos:definition  "received Time of an Asset"@en ;
        skos:prefLabel   "received At Time"@en .

rami:hasEnergyValue  a  owl:DatatypeProperty ;
        rdfs:domain     rami:CumulativeEnergyConsumption ;
        rdfs:range      xsd:float ;
        skos:prefLabel  "has Energy Value"@en .

dc:date  a      owl:AnnotationProperty .

dc:rights  a    owl:AnnotationProperty .

rami:hasDatatype  a   owl:ObjectProperty ;
        rdfs:comment  "Points to the datatypes of the Submodels"@en ;
        rdfs:domain   rami:Submodel ;
        rdfs:label    "has Datatype"@en .

dcterms:description  a  owl:AnnotationProperty .

rami:ComponentManager
        a           owl:Class ;
        rdfs:label  "Component Manager"@en .

foaf:Image  a   owl:Class .

rami:ITLayerDimension
        a                    owl:Class ;
        rdfs:label           "RAMI IT Layer Dimension"@en ;
        rdfs:subClassOf      rami:Dimension ;
        owl:equivalentClass  [ a          owl:Class ;
                               owl:oneOf  ( rami:Asset rami:Business rami:Communication rami:Functional rami:Information rami:Integration )
                             ] .

rami:Confirmation  a  owl:NamedIndividual , rami:ExpressionSemantic ;
        rdfs:comment  "For responses to requests that describe the capability of an asset."@en ;
        rdfs:label    "Confirmation"@en .

rami:hasValue  a      owl:ObjectProperty ;
        rdfs:comment  "Points to the current value that can be specified through an instanced submodel (for \ninstance in station 2) or through the asset."@en ;
        rdfs:domain   rami:Submodel ;
        rdfs:label    "has Value"@en ;
        rdfs:range    rami:Value .

rami:publishedURL  a  owl:DatatypeProperty .

dc:title  a     owl:AnnotationProperty .

rami:releaseDate  a      owl:DatatypeProperty ;
        rdfs:range       xsd:date ;
        skos:definition  "Release Date of the Standard"@en ;
        skos:prefLabel   "Release Date"@en .

xsd:date  a     rdfs:Datatype .

rami:Platform1  a  owl:NamedIndividual .

rami:hasRAMIHierarchyLevel
        a                owl:ObjectProperty ;
        rdfs:range       rami:HierarchyLevelDimension ;
        skos:definition  "Connects the concepts with the correspondent layer in the RAMI Hierarchy Levels"@en ;
        skos:prefLabel   "has RAMI Hierarchy Level"@en .

rami:Information  a  owl:NamedIndividual .

geo:long  a           owl:DatatypeProperty ;
        rdfs:comment  "The WGS84 longitude of a SpatialThing (decimal degrees)."@en ;
        rdfs:domain   rami:Machine ;
        rdfs:label    "long"@en ;
        rdfs:range    xsd:decimal .

dc:type  a      owl:AnnotationProperty .

rami:Asset2  a           owl:NamedIndividual , rami:Asset ;
        rdfs:label       "Asset 2"@en ;
        rami:hasAssetId  "AS712" .

rami:hasReference  a  owl:ObjectProperty ;
        rdfs:domain  rami:Submodel ;
        rdfs:label   "has Reference"@en .

rami:hasComponentManager
        a            owl:ObjectProperty ;
        rdfs:domain  rami:AdminShell ;
        rdfs:label   "has Component Manager"@en ;
        rdfs:range   rami:ComponentManager .

foaf:image  a         owl:DatatypeProperty , owl:AnnotationProperty ;
        rdfs:comment  "Image of the Asset reused from the FOAF ontology."@en ;
        rdfs:domain   rami:Asset ;
        rdfs:label    "image"@en ;
        rdfs:range    xsd:anyURI .

rami:EnergyEfficiency2
        a                           owl:NamedIndividual , rami:EnergyEfficiency ;
        rdfs:label                  "Energy Efficiency 2 Submodel"@en ;
        rami:energyEfficiencyValue  rami:MeasureEnergyEfficiency2 ;
        rami:subModelID             "AAB013" .

rami:inventoryNumber  a  owl:FunctionalProperty , owl:DatatypeProperty ;
        rdfs:domain      rami:Asset ;
        rdfs:range       xsd:string ;
        skos:definition  "Inventory number of the Entity/Object according to the identification nomenclature"@en ;
        skos:prefLabel   "Inventory Number"@en .

rami:TransportInterface
        a                owl:Class ;
        rdfs:subClassOf  rami:Submodel .

[ a            owl:AllDisjointClasses ;
  owl:members  ( rami:HierarchyLevelDimension rami:ITLayerDimension rami:LifeCycleDimension )
] .
