@prefix atm:      <https://data.nasa.gov/ontologies/atmonto/> .
@prefix bf:       <http://id.loc.gov/ontologies/bibframe/> .
@prefix bibo:     <http://purl.org/ontology/bibo/> .
@prefix dcterms:  <http://purl.org/dc/terms/> .
@prefix identity: <http://www.identity.org/ontologies/> .
@prefix igeo:     <http://rdf.insee.fr/def/> .
@prefix lswpm:    <http://ontology.cybershare.utep.edu/ELSEWeb/> .
@prefix npg:      <http://ns.nature.com/terms/> .
@prefix ore:      <http://www.openarchives.org/ore/terms/> .
@prefix ql:       <http://semweb.mmlab.be/ns/ql#> .
@prefix rml:      <http://semweb.mmlab.be/ns/rml#> .
@prefix rr:       <http://www.w3.org/ns/r2rml#> .
@prefix spcm:     <http://spi-fm.uca.es/spdef/models/deployment/spcm/> .

<https://w3id.org/i40/rami#SensorMeasurementData>
        a       <http://www.w3.org/2002/07/owl#Class> ;
        <http://www.w3.org/2000/01/rdf-schema#comment>
                "Data measured by a sensor"@en ;
        <http://www.w3.org/2000/01/rdf-schema#label>
                "Sensor Data"@en .

<https://w3id.org/i40/rami#subModelID>
        a       <http://www.w3.org/2002/07/owl#FunctionalProperty> , <http://www.w3.org/2002/07/owl#DatatypeProperty> ;
        <http://www.w3.org/2000/01/rdf-schema#comment>
                "Unique Identification for a Submodel"@en ;
        <http://www.w3.org/2000/01/rdf-schema#domain>
                <https://w3id.org/i40/rami#Submodel> ;
        <http://www.w3.org/2000/01/rdf-schema#label>
                "sub Model Id"@en ;
        <http://www.w3.org/2000/01/rdf-schema#range>
                <http://www.w3.org/2001/XMLSchema#string> ;
        <http://www.w3.org/2000/01/rdf-schema#subPropertyOf>
                dcterms:identifier .

<https://w3id.org/i40/rami#Submodel>
        a       <http://www.w3.org/2002/07/owl#Class> ;
        <http://www.w3.org/2000/01/rdf-schema#comment>
                "Describe the different types of Data related to the I4.0 Asset"@en ;
        <http://www.w3.org/2000/01/rdf-schema#label>
                "Submodel"@en .

dcterms:identifier  a  <http://www.w3.org/2002/07/owl#DatatypeProperty> , <http://www.w3.org/2002/07/owl#AnnotationProperty> ;
        <http://www.w3.org/2000/01/rdf-schema#range>
                <http://www.w3.org/2000/01/rdf-schema#Literal> ;
        <http://www.w3.org/2000/01/rdf-schema#subPropertyOf>
                <http://purl.org/dc/elements/1.1/identifier> .

<http://www.w3.org/2004/02/skos/core#note>
        a       <http://www.w3.org/2002/07/owl#AnnotationProperty> .

<http://purl.org/dc/elements/1.1/publisher>
        a       <http://www.w3.org/2002/07/owl#AnnotationProperty> .

<https://w3id.org/i40/rami#Value>
        a       <http://www.w3.org/2002/07/owl#Class> ;
        <http://www.w3.org/2000/01/rdf-schema#comment>
                "Current value that can be specified through an instanced submodel (for \ninstance in station 2) or through the asset, for example."@en ;
        <http://www.w3.org/2000/01/rdf-schema#label>
                "Value"@en .

<https://w3id.org/i40/rami#contributes>
        a       <http://www.w3.org/2002/07/owl#ObjectProperty> ;
        <http://www.w3.org/2000/01/rdf-schema#domain>
                <https://w3id.org/i40/rami#Submodel> ;
        <http://www.w3.org/2000/01/rdf-schema#range>
                <http://www.w3.org/ns/prov#Agent> ;
        <http://www.w3.org/2004/02/skos/core#definition>
                "Agent(Person or Software) that contributes to the Entity/Object related data. It correspond to the Contributor concept of OMM"@en ;
        <http://www.w3.org/2004/02/skos/core#prefLabel>
                "has Type Description"@en .

<http://www.w3.org/ns/prov#Agent>
        a       <http://www.w3.org/2002/07/owl#Class> .

<http://www.w3.org/2004/02/skos/core#definition>
        a       <http://www.w3.org/2002/07/owl#AnnotationProperty> .

<http://www.w3.org/2004/02/skos/core#prefLabel>
        a       <http://www.w3.org/2002/07/owl#AnnotationProperty> .

<https://w3id.org/i40/rami#I4.0Component1>
        a       <https://w3id.org/i40/rami#I4.0Component> , <http://www.w3.org/2002/07/owl#NamedIndividual> ;
        <http://www.w3.org/2000/01/rdf-schema#label>
                "I4.0 Component 2"@en ;
        <https://w3id.org/i40/rami#containsAS>
                <https://w3id.org/i40/rami#AdminShell2> ;
        <https://w3id.org/i40/rami#hasI40ComponentId>
                "I40C112" .

<https://w3id.org/i40/rami#I4.0Component>
        a       <http://www.w3.org/2002/07/owl#Class> ;
        <http://www.w3.org/2000/01/rdf-schema#comment>
                "Globally uniquely identifiable participant with communication capability consisting of administration shell and asset within an I4.0 system. \nSource: Industrie 4.0 – Begriffe/Terms, VDI Statusreport Industrie 4.0 (April 2017)"@en ;
        <http://www.w3.org/2000/01/rdf-schema#isDefinedBy>
                "https://www.plattform-i40.de/I40/Navigation/EN/Service/Glossary/glossary.html" ;
        <http://www.w3.org/2000/01/rdf-schema#label>
                "I4.0Component"@en ;
        <http://www.w3.org/2002/07/owl#equivalentClass>
                [ a       <http://www.w3.org/2002/07/owl#Restriction> ;
                  <http://www.w3.org/2002/07/owl#minQualifiedCardinality>
                          1 ;
                  <http://www.w3.org/2002/07/owl#onClass>
                          <https://w3id.org/i40/rami#AdminShell> ;
                  <http://www.w3.org/2002/07/owl#onProperty>
                          <https://w3id.org/i40/rami#containsAS>
                ] .

<https://w3id.org/i40/rami#containsAS>
        a       <http://www.w3.org/2002/07/owl#ObjectProperty> ;
        <http://www.w3.org/2000/01/rdf-schema#comment>
                "Points the I4.0 Component to the Administration Shell"@en ;
        <http://www.w3.org/2000/01/rdf-schema#domain>
                <https://w3id.org/i40/rami#I4.0Component> ;
        <http://www.w3.org/2000/01/rdf-schema#label>
                "contains Admin Shell"@en ;
        <http://www.w3.org/2000/01/rdf-schema#range>
                <https://w3id.org/i40/rami#AdminShell> .

<https://w3id.org/i40/rami#AdminShell2>
        a       <http://www.w3.org/2002/07/owl#NamedIndividual> , <https://w3id.org/i40/rami#AdminShell> ;
        <http://www.w3.org/2000/01/rdf-schema#label>
                "Admin Shell 2"@en ;
        <https://w3id.org/i40/rami#hasAdminShellId>
                "AAS112" ;
        <https://w3id.org/i40/rami#hasSubmodel>
                <https://w3id.org/i40/rami#EnergyEfficiency2> .

<https://w3id.org/i40/rami#hasI40ComponentId>
        a       <http://www.w3.org/2002/07/owl#FunctionalProperty> , <http://www.w3.org/2002/07/owl#DatatypeProperty> ;
        <http://www.w3.org/2000/01/rdf-schema#comment>
                "Unique Identification of the Industry 4.0 component."@en ;
        <http://www.w3.org/2000/01/rdf-schema#domain>
                <https://w3id.org/i40/rami#I4.0Component> ;
        <http://www.w3.org/2000/01/rdf-schema#label>
                "has I40 Component Id"@en ;
        <http://www.w3.org/2000/01/rdf-schema#range>
                <http://www.w3.org/2001/XMLSchema#string> ;
        <http://www.w3.org/2000/01/rdf-schema#subPropertyOf>
                dcterms:identifier .

<http://purl.org/dc/elements/1.1/coverage>
        a       <http://www.w3.org/2002/07/owl#AnnotationProperty> .

<https://w3id.org/i40/rami#Business>
        a       <http://www.w3.org/2002/07/owl#NamedIndividual> .

<https://w3id.org/i40/rami#AdminShell>
        a       <http://www.w3.org/2002/07/owl#Class> ;
        <http://www.w3.org/2000/01/rdf-schema#label>
                "Admin Shell"@en ;
        <http://purl.org/dc/elements/1.1/source>
                "This definition comprises material from RAMI4.0."@en ;
        <http://www.w3.org/2004/02/skos/core#altLabel>
                "Asset Administration Shell"@en , "Administration Shell"@en ;
        <http://www.w3.org/2004/02/skos/core#definition>
                "Describes the Administration Shell for Assets, Products, Components, e.g. Machines"@en ;
        <http://www.w3.org/2004/02/skos/core#prefLabel>
                "Verwaltungsschale"@de .

<https://w3id.org/i40/rami#TechnicalData1>
        a       <http://www.w3.org/2002/07/owl#NamedIndividual> ;
        <http://www.w3.org/2000/01/rdf-schema#label>
                "Technical Data 1"@en ;
        <https://w3id.org/i40/rami#display>
                "Seven-segment display"@en .

<https://w3id.org/i40/rami#display>
        a       <http://www.w3.org/2002/07/owl#AnnotationProperty> .

<http://www.w3.org/2004/02/skos/core#example>
        a       <http://www.w3.org/2002/07/owl#AnnotationProperty> .

<https://w3id.org/i40/rami#usesStandard>
        a       <http://www.w3.org/2002/07/owl#ObjectProperty> ;
        <http://www.w3.org/2000/01/rdf-schema#comment>
                "Points to the standards describing the functions attached to the asset via the administration shell"@en ;
        <http://www.w3.org/2000/01/rdf-schema#label>
                "uses Standard"@en ;
        <http://www.w3.org/2000/01/rdf-schema#range>
                <https://w3id.org/i40/sto#Standard> .

<https://w3id.org/i40/sto#Standard>
        a       <http://www.w3.org/2002/07/owl#Class> ;
        <http://www.w3.org/2000/01/rdf-schema#isDefinedBy>
                <https://w3id.org/i40/sto/#Standard> ;
        <http://www.w3.org/2004/02/skos/core#definition>
                "Standards that are used to describe the actual I4.0 Asset. Defined in the STO ontology"@en ;
        <http://www.w3.org/2004/02/skos/core#prefLabel>
                "Standard"@en .

<https://w3id.org/i40/rami#Structure>
        a       <http://www.w3.org/2002/07/owl#Class> ;
        <http://www.w3.org/2000/01/rdf-schema#subClassOf>
                <https://w3id.org/i40/rami#Submodel> .

<https://w3id.org/i40/rami#BrakingResistanceMs>
        a       <http://www.w3.org/2002/07/owl#NamedIndividual> , <http://www.wurvoc.org/vocabularies/om-1.8/Measure> ;
        <http://www.wurvoc.org/vocabularies/om-1.8/hasNumericalValue>
                "60.0"^^<http://www.w3.org/2001/XMLSchema#float> ;
        <http://www.wurvoc.org/vocabularies/om-1.8/hasUnit>
                <http://www.wurvoc.org/vocabularies/om-1.8/ohm> .

<http://www.wurvoc.org/vocabularies/om-1.8/Measure>
        a       <http://www.w3.org/2002/07/owl#Class> .

<http://www.wurvoc.org/vocabularies/om-1.8/hasNumericalValue>
        a       <http://www.w3.org/2002/07/owl#DatatypeProperty> , <http://www.w3.org/2002/07/owl#AnnotationProperty> ;
        <http://www.w3.org/2000/01/rdf-schema#domain>
                <http://www.wurvoc.org/vocabularies/om-1.8/Measure> ;
        <http://www.w3.org/2000/01/rdf-schema#label>
                "has numerical value"@en .

<http://www.wurvoc.org/vocabularies/om-1.8/hasUnit>
        a       <http://www.w3.org/2002/07/owl#ObjectProperty> ;
        <http://www.w3.org/2000/01/rdf-schema#domain>
                <http://www.wurvoc.org/vocabularies/om-1.8/Measure> ;
        <http://www.w3.org/2000/01/rdf-schema#label>
                "has unit"@en ;
        <http://www.w3.org/2000/01/rdf-schema#range>
                <http://www.wurvoc.org/vocabularies/om-1.8/Unit> .

<http://www.wurvoc.org/vocabularies/om-1.8/ohm>
        a       <http://www.w3.org/2002/07/owl#NamedIndividual> .

<https://w3id.org/i40/rami#hasSemanticExpression>
        a       <http://www.w3.org/2002/07/owl#ObjectProperty> ;
        <http://www.w3.org/2000/01/rdf-schema#comment>
                "Points to the Expression Semantic of the Submodels"@en ;
        <http://www.w3.org/2000/01/rdf-schema#domain>
                <https://w3id.org/i40/rami#Submodel> ;
        <http://www.w3.org/2000/01/rdf-schema#label>
                "has Semantic Expression"@en ;
        <http://www.w3.org/2000/01/rdf-schema#range>
                <https://w3id.org/i40/rami#ExpressionSemantic> .

<https://w3id.org/i40/rami#ExpressionSemantic>
        a       <http://www.w3.org/2002/07/owl#Class> ;
        <http://www.w3.org/2000/01/rdf-schema#comment>
                "Specifies which role the property plays in an interaction, i.e. which \nexpression the provider of the property intends. \nValid values are: Requirement (for requests that are to be confirmed or rejected) Confirmations (for responses to requests that describe the capability of an asset) Measurement (if a measured or actual value is provided)"@en ;
        <http://www.w3.org/2000/01/rdf-schema#isDefinedBy>
                "https://www.zvei.org/fileadmin/user_upload/Presse_und_Medien/Publikationen/2017/April/Asset_Administration_Shell/ZVEI_WP_Verwaltungschale_Englisch_Download_03.04.17.pdf" ;
        <http://www.w3.org/2000/01/rdf-schema#label>
                "Expression Semantic"@en , "Ausprägungsaussage"@de ;
        <http://www.w3.org/2002/07/owl#equivalentClass>
                [ a       <http://www.w3.org/2002/07/owl#Class> ;
                  <http://www.w3.org/2002/07/owl#oneOf>
                          ( <https://w3id.org/i40/rami#Confirmation> <https://w3id.org/i40/rami#Measurement> <https://w3id.org/i40/rami#Requirement> )
                ] .

<https://w3id.org/i40/rami#Reference>
        a       <http://www.w3.org/2002/07/owl#Class> .

<https://w3id.org/i40/rami#Function>
        a       <http://www.w3.org/2002/07/owl#NamedIndividual> , <https://w3id.org/i40/rami#View> ;
        <http://www.w3.org/2000/01/rdf-schema#comment>
                "Makes statements on the function pursuant to IEC 81346 and on the function of the asset components.\nIncludes skills such as interpretation (?), commissioning, calculation (?) or diagnosis functions of the asset.\nExamples: current imbalance detection ability"@en ;
        <http://www.w3.org/2000/01/rdf-schema#label>
                "Function"@en .

<https://w3id.org/i40/rami#View>
        a       <http://www.w3.org/2002/07/owl#Class> ;
        <http://www.w3.org/2000/01/rdf-schema#comment>
                "Different views associated to the Administration Shell via the Submodels"@en ;
        <http://www.w3.org/2000/01/rdf-schema#isDefinedBy>
                "https://www.plattform-i40.de/I40/Redaktion/DE/Downloads/Publikation/hm-2018-trilaterale-coop.html"@de ;
        <http://www.w3.org/2000/01/rdf-schema#label>
                "View" , "Sicht"@de ;
        <http://www.w3.org/2002/07/owl#equivalentClass>
                [ a       <http://www.w3.org/2002/07/owl#Class> ;
                  <http://www.w3.org/2002/07/owl#oneOf>
                          ( <https://w3id.org/i40/rami#BusinessView> <https://w3id.org/i40/rami#Construction> <https://w3id.org/i40/rami#Function> <https://w3id.org/i40/rami#Location> <https://w3id.org/i40/rami#Performance> )
                ] .

dcterms:hasVersion  a  <http://www.w3.org/2002/07/owl#AnnotationProperty> .

<http://www.w3.org/2004/02/skos/core#narrower>
        a       <http://www.w3.org/2002/07/owl#AnnotationProperty> .

<https://w3id.org/i40/rami#energyEfficiencyValue>
        a       <http://www.w3.org/2002/07/owl#ObjectProperty> ;
        <http://www.w3.org/2000/01/rdf-schema#comment>
                "Points to the value of the Energy Efficiency comsuption."@en ;
        <http://www.w3.org/2000/01/rdf-schema#domain>
                <https://w3id.org/i40/rami#EnergyEfficiency> ;
        <http://www.w3.org/2000/01/rdf-schema#label>
                "energy Efficiency Value"@en ;
        <http://www.w3.org/2000/01/rdf-schema#range>
                <http://www.wurvoc.org/vocabularies/om-1.8/Measure> .

<https://w3id.org/i40/rami#EnergyEfficiency>
        a       <http://www.w3.org/2002/07/owl#Class> ;
        <http://www.w3.org/2000/01/rdf-schema#subClassOf>
                <https://w3id.org/i40/rami#Submodel> .

<http://purl.org/dc/elements/1.1/identifier>
        a       <http://www.w3.org/2002/07/owl#AnnotationProperty> .

<http://www.wurvoc.org/vocabularies/om-1.8/Unit>
        a       <http://www.w3.org/2002/07/owl#Class> .

<http://purl.org/dc/elements/1.1/language>
        a       <http://www.w3.org/2002/07/owl#AnnotationProperty> .

<https://w3id.org/i40/rami#hasAssetId>
        a       <http://www.w3.org/2002/07/owl#FunctionalProperty> , <http://www.w3.org/2002/07/owl#DatatypeProperty> ;
        <http://www.w3.org/2000/01/rdf-schema#comment>
                "Unique identification for the Asset."@en ;
        <http://www.w3.org/2000/01/rdf-schema#domain>
                <https://w3id.org/i40/rami#Asset> ;
        <http://www.w3.org/2000/01/rdf-schema#label>
                "has Asset Id"@en ;
        <http://www.w3.org/2000/01/rdf-schema#range>
                <http://www.w3.org/2001/XMLSchema#string> ;
        <http://www.w3.org/2000/01/rdf-schema#subPropertyOf>
                dcterms:identifier .

<https://w3id.org/i40/rami#Asset>
        a       <http://www.w3.org/2002/07/owl#Class> , <http://www.w3.org/2002/07/owl#NamedIndividual> ;
        <http://www.w3.org/2004/02/skos/core#altLabel>
                "Entität"@de , "Entity"@en , "Object"@en ;
        <http://www.w3.org/2004/02/skos/core#definition>
                "Eindeutig identifizierbarer Gegenstand, der aufgrund seiner Bedeutung in der Informationswelt verwaltet wird"@de , "Clearly identifiable asset for the Administration Shell"@en ;
        <http://www.w3.org/2004/02/skos/core#note>
                "Objects may be known in the form of a type or of an instance. An object in the planning phase is known as a type"@en ;
        <http://www.w3.org/2004/02/skos/core#prefLabel>
                "Asset"@en .

<https://w3id.org/i40/rami#Requirement>
        a       <http://www.w3.org/2002/07/owl#NamedIndividual> , <https://w3id.org/i40/rami#ExpressionSemantic> ;
        <http://www.w3.org/2000/01/rdf-schema#comment>
                "For requests that are to be confirmed or rejected"@en ;
        <http://www.w3.org/2000/01/rdf-schema#label>
                "Requirement"@en .

<https://w3id.org/i40/rami#hasData>
        a       <http://www.w3.org/2002/07/owl#ObjectProperty> ;
        <http://www.w3.org/2000/01/rdf-schema#domain>
                <https://w3id.org/i40/rami#AdminShell> ;
        <http://www.w3.org/2000/01/rdf-schema#range>
                <https://w3id.org/i40/rami#Submodel> ;
        <http://www.w3.org/2004/02/skos/core#definition>
                "Connects the AdminShell with the different types of Data for the Object/Entity"@en ;
        <http://www.w3.org/2004/02/skos/core#prefLabel>
                "has Data"@en .

<https://w3id.org/i40/rami#Construction>
        a       <http://www.w3.org/2002/07/owl#NamedIndividual> , <https://w3id.org/i40/rami#View> ;
        <http://www.w3.org/2000/01/rdf-schema#comment>
                "Applies to the constructive deployment of the asset for selection, design of building structure or assemblies ...\nContains a structure classification system pursuant to IEC 81346.\nApplies to properties in respect of:\n1) physical dimensions and regarding start, processing and output values of the component.\n2) modular view of subcomponents or a asset structure and 3) inputs and outputs of different signal types."@en ;
        <http://www.w3.org/2000/01/rdf-schema#label>
                "Construction"@en .

<https://w3id.org/i40/rami#LifeCycleDimension>
        a       <http://www.w3.org/2002/07/owl#Class> ;
        <http://www.w3.org/2000/01/rdf-schema#label>
                "RAMI Life Cycle Dimension"@en ;
        <http://www.w3.org/2000/01/rdf-schema#seeAlso>
                "http://www.zvei.org/en/subjects/Industry-40/Pages/The-Reference-Architectural-Model-RAMI-40-and-the-Industrie-40-Component.aspx" ;
        <http://www.w3.org/2000/01/rdf-schema#seeAlso>
                <http://www.zvei.org/en/subjects/Industry-40/Pages/The-Reference-Architectural-Model-RAMI-40-and-the-Industrie-40-Component.aspx> ;
        <http://www.w3.org/2000/01/rdf-schema#subClassOf>
                <https://w3id.org/i40/rami#Dimension> ;
        <http://www.w3.org/2002/07/owl#equivalentClass>
                [ a       <http://www.w3.org/2002/07/owl#Class> ;
                  <http://www.w3.org/2002/07/owl#oneOf>
                          ( <https://w3id.org/i40/rami#Instance> <https://w3id.org/i40/rami#Type> )
                ] ;
        <http://www.w3.org/2004/02/skos/core#definition>
                "It describes the different Life Cycle and Value Stream layers for the RAMI model according to the IEC 62890 Standard."@en ;
        <http://www.w3.org/2004/02/skos/core#prefLabel>
                "RAMI Life Cycle Dimension"@en , "RAMI Layer"@en .

<https://w3id.org/i40/rami#Dimension>
        a       <http://www.w3.org/2002/07/owl#Class> ;
        <http://www.w3.org/2000/01/rdf-schema#comment>
                "Abstract class to describe the three different dimensions of RAMI4.0"@en ;
        <http://www.w3.org/2000/01/rdf-schema#label>
                "Dimension"@en .

<https://w3id.org/i40/rami#Instance>
        a       <http://www.w3.org/2002/07/owl#NamedIndividual> , <https://w3id.org/i40/rami#LifeCycleDimension> .

<https://w3id.org/i40/rami#Type>
        a       <http://www.w3.org/2002/07/owl#NamedIndividual> , <https://w3id.org/i40/rami#LifeCycleDimension> ;
        <http://www.w3.org/2000/01/rdf-schema#label>
                "Type"@en .

<https://w3id.org/i40/rami#MeasureEnergyEfficiency1>
        a       <http://www.w3.org/2002/07/owl#NamedIndividual> , <http://www.wurvoc.org/vocabularies/om-1.8/Measure> ;
        <http://www.w3.org/2000/01/rdf-schema#comment>
                "Measuring the Energy Efficiency for I4.0 component 1 in kilowattHour."@en ;
        <http://www.w3.org/2000/01/rdf-schema#label>
                "Measure Energy Efficiency 1"@en ;
        <http://www.w3.org/2002/07/owl#sameAs>
                <https://w3id.org/i40/rami#MeasureEnergyEfficiency2> ;
        <http://www.wurvoc.org/vocabularies/om-1.8/hasNumericalValue>
                "17.3"^^<http://www.w3.org/2001/XMLSchema#float> ;
        <http://www.wurvoc.org/vocabularies/om-1.8/hasUnit>
                <http://www.wurvoc.org/vocabularies/om-1.8/kilowattHour> .

<https://w3id.org/i40/rami#MeasureEnergyEfficiency2>
        a       <http://www.w3.org/2002/07/owl#NamedIndividual> , <http://www.wurvoc.org/vocabularies/om-1.8/Measure> ;
        <http://www.w3.org/2000/01/rdf-schema#comment>
                "Measuring the Energy Efficiency for I4.0 component 2 in Kilojoule."@en ;
        <http://www.w3.org/2000/01/rdf-schema#label>
                "Measure Energy Efficiency 2"@en ;
        <http://www.wurvoc.org/vocabularies/om-1.8/hasNumericalValue>
                "62280.0"^^<http://www.w3.org/2001/XMLSchema#float> ;
        <http://www.wurvoc.org/vocabularies/om-1.8/hasUnit>
                <http://www.wurvoc.org/vocabularies/om-1.8/kilojoule> .

<http://www.wurvoc.org/vocabularies/om-1.8/kilowattHour>
        a       <http://www.w3.org/2002/07/owl#NamedIndividual> .

<http://www.loa-cnr.it/ontologies/DUL.owl#isPartOf>
        a       <http://www.w3.org/2002/07/owl#ObjectProperty> , <http://www.w3.org/2002/07/owl#TransitiveProperty> ;
        <http://www.w3.org/2000/01/rdf-schema#comment>
                "A relation between any entities, in this case, the Asset can be part of other Asset(s)." ;
        <http://www.w3.org/2000/01/rdf-schema#domain>
                <https://w3id.org/i40/rami#Asset> ;
        <http://www.w3.org/2000/01/rdf-schema#isDefinedBy>
                <http://www.ontologydesignpatterns.org/ont/dul/DUL.owl> ;
        <http://www.w3.org/2000/01/rdf-schema#label>
                "is Part Of"@en ;
        <http://www.w3.org/2000/01/rdf-schema#range>
                <https://w3id.org/i40/rami#Asset> .

<https://w3id.org/i40/rami#Platform>
        a       <http://www.w3.org/2002/07/owl#Class> .

<https://w3id.org/i40/rami#MESConnection>
        a       <http://www.w3.org/2002/07/owl#Class> ;
        <http://www.w3.org/2000/01/rdf-schema#subClassOf>
                <https://w3id.org/i40/rami#Submodel> .

<http://www.w3.org/2004/02/skos/core#altLabel>
        a       <http://www.w3.org/2002/07/owl#AnnotationProperty> .

<https://w3id.org/i40/rami#maxOutputFrequencyMs>
        a       <http://www.w3.org/2002/07/owl#NamedIndividual> , <http://www.wurvoc.org/vocabularies/om-1.8/Measure> ;
        <http://www.wurvoc.org/vocabularies/om-1.8/hasNumericalValue>
                "1.0"^^<http://www.w3.org/2001/XMLSchema#float> ;
        <http://www.wurvoc.org/vocabularies/om-1.8/hasUnit>
                <http://www.wurvoc.org/vocabularies/om-1.8/hertz> .

<http://www.wurvoc.org/vocabularies/om-1.8/hertz>
        a       <http://www.w3.org/2002/07/owl#NamedIndividual> .

<http://purl.org/dc/elements/1.1/subject>
        a       <http://www.w3.org/2002/07/owl#AnnotationProperty> .

<https://w3id.org/i40/rami#Station>
        a       <http://www.w3.org/2002/07/owl#NamedIndividual> , <https://w3id.org/i40/rami#HierarchyLevelDimension> ;
        <http://www.w3.org/2004/02/skos/core#definition>
                "Station hierarchy level of RAMI 4.0"@en ;
        <http://www.w3.org/2004/02/skos/core#prefLabel>
                "Station"@en .

<https://w3id.org/i40/rami#HierarchyLevelDimension>
        a       <http://www.w3.org/2002/07/owl#Class> ;
        <http://www.w3.org/2000/01/rdf-schema#seeAlso>
                <http://www.zvei.org/en/subjects/Industry-40/Pages/The-Reference-Architectural-Model-RAMI-40-and-the-Industrie-40-Component.aspx> ;
        <http://www.w3.org/2000/01/rdf-schema#subClassOf>
                <https://w3id.org/i40/rami#Dimension> ;
        <http://www.w3.org/2002/07/owl#equivalentClass>
                [ a       <http://www.w3.org/2002/07/owl#Class> ;
                  <http://www.w3.org/2002/07/owl#oneOf>
                          ( <https://w3id.org/i40/rami#ConnectedWorld> <https://w3id.org/i40/rami#ControlDevice> <https://w3id.org/i40/rami#Enterprise> <https://w3id.org/i40/rami#FieldDevice> <https://w3id.org/i40/rami#Product> <https://w3id.org/i40/rami#Station> <https://w3id.org/i40/rami#WorkCenter> )
                ] ;
        <http://www.w3.org/2004/02/skos/core#definition>
                "It describes the functional classification of various circumstances within Industrie 4.0. For classification within a factory, this axis of the reference architecture(layers) follows the IEC 62264 Standard."@en ;
        <http://www.w3.org/2004/02/skos/core#prefLabel>
                "RAMI Hierarchy Level Dimension"@en .

<https://w3id.org/i40/rami#isDescribedWith>
        a       <http://www.w3.org/2002/07/owl#DatatypeProperty> , <http://www.w3.org/2002/07/owl#ObjectProperty> ;
        <http://www.w3.org/2000/01/rdf-schema#domain>
                <https://w3id.org/i40/rami#AdminShell> ;
        <http://www.w3.org/2000/01/rdf-schema#range>
                <https://w3id.org/i40/sto#Standard> ;
        <http://www.w3.org/2004/02/skos/core#definition>
                "Points to the Standard used to describe a given object"@en ;
        <http://www.w3.org/2004/02/skos/core#prefLabel>
                "Is Described With"@en .

<https://w3id.org/i40/rami#WorkCenter>
        a       <http://www.w3.org/2002/07/owl#NamedIndividual> , <https://w3id.org/i40/rami#HierarchyLevelDimension> ;
        <http://www.w3.org/2004/02/skos/core#definition>
                "Work Center hierarchy level of RAMI 4.0"@en ;
        <http://www.w3.org/2004/02/skos/core#prefLabel>
                "Work Center"@en .

<https://w3id.org/i40/rami#hasManifest>
        a       <http://www.w3.org/2002/07/owl#ObjectProperty> ;
        <http://www.w3.org/2000/01/rdf-schema#domain>
                <https://w3id.org/i40/rami#AdminShell> ;
        <http://www.w3.org/2000/01/rdf-schema#label>
                "has Manifest"@en ;
        <http://www.w3.org/2000/01/rdf-schema#range>
                <https://w3id.org/i40/rami#Manifest> .

<https://w3id.org/i40/rami#Manifest>
        a       <http://www.w3.org/2002/07/owl#Class> ;
        <http://www.w3.org/2000/01/rdf-schema#label>
                "Manifest"@en .

<https://w3id.org/i40/rami#>
        a       <http://www.w3.org/2002/07/owl#Ontology> ;
        <http://www.w3.org/2000/01/rdf-schema#isDefinedBy>
                <https://w3id.org/i40/rami#> ;
        <http://purl.org/vocab/vann/preferredNamespacePrefix>
                "rami" ;
        <http://purl.org/vocab/vann/preferredNamespaceUri>
                "https://w3id.org/i40/rami#" ;
        <http://rdfs.org/ns/void#vocabulary>
                <http://www.w3.org/2001/XMLSchema#> , <http://xmlns.com/foaf/spec/> , <http://www.w3.org/2000/01/rdf-schema#> , <http://www.w3.org/XML/1998/namespace> , <http://www.w3.org/2004/02/skos/core#> , <http://www.w3.org/1999/02/22-rdf-syntax-ns#> , <http://purl.org/dc/elements/1.1/> ;
        <http://www.w3.org/2002/07/owl#versionInfo>
                "0.3" ;
        <http://www.w3.org/2004/02/skos/core#definition>
                "An Ontology to represents the Reference Architecture Model for Industry 4.0 (RAMI), including the concept of the Administration Shell I4.0 Component."@en ;
        <http://www.w3.org/2004/02/skos/core#prefLabel>
                "rami"@en .

<https://w3id.org/i40/rami#creationDate>
        a       <http://www.w3.org/2002/07/owl#DatatypeProperty> ;
        <http://www.w3.org/2000/01/rdf-schema#domain>
                <https://w3id.org/i40/rami#Submodel> ;
        <http://www.w3.org/2000/01/rdf-schema#range>
                <http://www.w3.org/2001/XMLSchema#dateTime> ;
        <http://www.w3.org/2004/02/skos/core#definition>
                "Date when an Agent(Person or Software) creates to the Entity/Object related data. It correspond to the Creator concept of OMM"@en ;
        <http://www.w3.org/2004/02/skos/core#prefLabel>
                "has Creator"@en .

<https://w3id.org/i40/rami#Product>
        a       <http://www.w3.org/2002/07/owl#NamedIndividual> , <https://w3id.org/i40/rami#HierarchyLevelDimension> ;
        <http://www.w3.org/2004/02/skos/core#definition>
                "Product hierarchy level of RAMI 4.0"@en ;
        <http://www.w3.org/2004/02/skos/core#prefLabel>
                "Product"@en .

<https://w3id.org/i40/rami#Integration>
        a       <http://www.w3.org/2002/07/owl#NamedIndividual> .

<http://www.w3.org/ns/prov#wasGeneratedBy>
        a       <http://www.w3.org/2002/07/owl#ObjectProperty> ;
        <http://www.w3.org/2000/01/rdf-schema#domain>
                <https://w3id.org/i40/rami#Submodel> ;
        <http://www.w3.org/2000/01/rdf-schema#range>
                <http://www.w3.org/ns/prov#Agent> ;
        <http://www.w3.org/2004/02/skos/core#definition>
                "Agent (Person or Software) that generates the Asset related data. It correspond to the Creator concept of OMM"@en ;
        <http://www.w3.org/2004/02/skos/core#prefLabel>
                "was Generated By"@en .

<https://w3id.org/i40/rami#Order>
        a       <http://www.w3.org/2002/07/owl#Class> ;
        <http://www.w3.org/2004/02/skos/core#definition>
                "Each order for manufacturing runs through a life cycle and its specifics necessarily have an impact on the production facility during performance of the order"@en ;
        <http://www.w3.org/2004/02/skos/core#prefLabel>
                "Order"@en .

<http://purl.org/dc/elements/1.1/relation>
        a       <http://www.w3.org/2002/07/owl#AnnotationProperty> .

<http://purl.org/dc/elements/1.1/creator>
        a       <http://www.w3.org/2002/07/owl#AnnotationProperty> .

<http://www.w3.org/2004/02/skos/core#hiddenLabel>
        a       <http://www.w3.org/2002/07/owl#AnnotationProperty> .

<http://purl.org/dc/elements/1.1/format>
        a       <http://www.w3.org/2002/07/owl#AnnotationProperty> .

<https://w3id.org/i40/rami#ConnectedWorld>
        a       <http://www.w3.org/2002/07/owl#NamedIndividual> , <https://w3id.org/i40/rami#HierarchyLevelDimension> ;
        <http://www.w3.org/2004/02/skos/core#definition>
                "Connected World hierarchy level of RAMI 4.0. Group of Factories, and the collaboration with external engineering firms, component suppliers and customers"@en ;
        <http://www.w3.org/2004/02/skos/core#prefLabel>
                "Connected World"@en .

<https://w3id.org/i40/rami#ControlDevice>
        a       <http://www.w3.org/2002/07/owl#NamedIndividual> , <https://w3id.org/i40/rami#HierarchyLevelDimension> ;
        <http://www.w3.org/2004/02/skos/core#definition>
                "Control Device hierarchy level of RAMI 4.0"@en ;
        <http://www.w3.org/2004/02/skos/core#prefLabel>
                "Control Device"@en .

<https://w3id.org/i40/rami#Enterprise>
        a       <http://www.w3.org/2002/07/owl#NamedIndividual> , <https://w3id.org/i40/rami#HierarchyLevelDimension> ;
        <http://www.w3.org/2004/02/skos/core#definition>
                "Enterprise hierarchy level of RAMI 4.0"@en ;
        <http://www.w3.org/2004/02/skos/core#prefLabel>
                "Enterprise"@en .

<https://w3id.org/i40/rami#FieldDevice>
        a       <http://www.w3.org/2002/07/owl#NamedIndividual> , <https://w3id.org/i40/rami#HierarchyLevelDimension> ;
        <http://www.w3.org/2004/02/skos/core#definition>
                "Field Device hierarchy level of RAMI 4.0"@en ;
        <http://www.w3.org/2004/02/skos/core#prefLabel>
                "Field Device"@en .

<https://w3id.org/i40/rami#CumulativeEnergyConsumption>
        a       <http://www.w3.org/2002/07/owl#Class> .

<https://w3id.org/i40/rami#inAccordanceWith>
        a       <http://www.w3.org/2002/07/owl#ObjectProperty> ;
        <http://www.w3.org/2000/01/rdf-schema#comment>
                "The Submodel is in accordance with a given standard specified in the STO ontology"@en ;
        <http://www.w3.org/2000/01/rdf-schema#domain>
                <https://w3id.org/i40/rami#Submodel> ;
        <http://www.w3.org/2000/01/rdf-schema#label>
                "in Accordance With"@en ;
        <http://www.w3.org/2000/01/rdf-schema#range>
                <https://w3id.org/i40/sto#Standard> .

<https://w3id.org/i40/rami#SensorMeasurement>
        a       <http://www.w3.org/2002/07/owl#Class> ;
        <http://www.w3.org/2000/01/rdf-schema#subClassOf>
                <https://w3id.org/i40/rami#Submodel> .

<https://w3id.org/i40/rami#I4.0Component2>
        a       <https://w3id.org/i40/rami#I4.0Component> , <http://www.w3.org/2002/07/owl#NamedIndividual> ;
        <http://www.w3.org/2000/01/rdf-schema#label>
                "I4.0 Component 1"@en ;
        <https://w3id.org/i40/rami#containsAS>
                <https://w3id.org/i40/rami#AdminShell1> ;
        <https://w3id.org/i40/rami#hasI40ComponentId>
                "I40C111" .

<https://w3id.org/i40/rami#AdminShell1>
        a       <http://www.w3.org/2002/07/owl#NamedIndividual> , <https://w3id.org/i40/rami#AdminShell> ;
        <http://www.w3.org/2000/01/rdf-schema#label>
                "Admin Shell 1"@en ;
        <https://w3id.org/i40/rami#hasAdminShellId>
                "AAS111" ;
        <https://w3id.org/i40/rami#hasSubmodel>
                <https://w3id.org/i40/rami#EnergyEfficiency1> .

<https://w3id.org/i40/rami#isConnectedTo>
        a       <http://www.w3.org/2002/07/owl#ObjectProperty> ;
        <http://www.w3.org/2000/01/rdf-schema#comment>
                "Connects the Admin Shell with the different RAMI4.0 Dimensions"@en ;
        <http://www.w3.org/2000/01/rdf-schema#domain>
                <https://w3id.org/i40/rami#AdminShell> ;
        <http://www.w3.org/2000/01/rdf-schema#label>
                "is Connected To"@en ;
        <http://www.w3.org/2000/01/rdf-schema#range>
                <https://w3id.org/i40/rami#Dimension> .

<https://w3id.org/i40/rami#Functional>
        a       <http://www.w3.org/2002/07/owl#NamedIndividual> .

<http://purl.org/dc/elements/1.1/source>
        a       <http://www.w3.org/2002/07/owl#AnnotationProperty> .

<https://w3id.org/i40/rami#AdminShellMotor>
        a       <http://www.w3.org/2002/07/owl#NamedIndividual> , <https://w3id.org/i40/rami#AdminShell> ;
        <http://www.w3.org/2000/01/rdf-schema#label>
                "Admin Shell Motor"@en ;
        <https://w3id.org/i40/rami#describes>
                <https://w3id.org/i40/rami#AssetMotorControl> .

<https://w3id.org/i40/rami#describes>
        a       <http://www.w3.org/2002/07/owl#ObjectProperty> ;
        <http://www.w3.org/2000/01/rdf-schema#comment>
                "Connect the Asset with the Administration Shell"@en ;
        <http://www.w3.org/2000/01/rdf-schema#domain>
                <https://w3id.org/i40/rami#AdminShell> ;
        <http://www.w3.org/2000/01/rdf-schema#label>
                "describes"@en ;
        <http://www.w3.org/2000/01/rdf-schema#range>
                <https://w3id.org/i40/rami#Asset> .

<https://w3id.org/i40/rami#AssetMotorControl>
        a       <http://www.w3.org/2002/07/owl#NamedIndividual> , <https://w3id.org/i40/rami#Asset> ;
        <http://www.w3.org/2000/01/rdf-schema#label>
                "Motor control"@en ;
        <https://w3id.org/i40/rami#hasAssetId>
                "1501325" .

<http://purl.org/dc/elements/1.1/description>
        a       <http://www.w3.org/2002/07/owl#AnnotationProperty> .

<https://w3id.org/i40/rami#Asset1>
        a       <http://www.w3.org/2002/07/owl#NamedIndividual> , <https://w3id.org/i40/rami#Asset> ;
        <http://www.w3.org/2000/01/rdf-schema#label>
                "Asset 1"@en ;
        <https://w3id.org/i40/rami#hasAssetId>
                "AS711" .

<https://w3id.org/i40/rami#Communication>
        a       <http://www.w3.org/2002/07/owl#NamedIndividual> .

<https://w3id.org/i40/rami#Machine>
        a       <http://www.w3.org/2002/07/owl#Class> ;
        <http://www.w3.org/2000/01/rdf-schema#subClassOf>
                <https://w3id.org/i40/rami#Asset> ;
        <http://www.w3.org/2004/02/skos/core#definition>
                "A machine is ordered, designed, commissioned, operated, serviced, converted and recycled."@en ;
        <http://www.w3.org/2004/02/skos/core#prefLabel>
                "Machine"@en .

<http://www.wurvoc.org/vocabularies/om-1.8/kilojoule>
        a       <http://www.w3.org/2002/07/owl#NamedIndividual> .

<http://purl.oclc.org/NET/ssnx/ssn#Sensor>
        a       <http://www.w3.org/2002/07/owl#Class> .

<http://www.w3.org/2003/01/geo/wgs84_pos#lat>
        a       <http://www.w3.org/2002/07/owl#DatatypeProperty> ;
        <http://www.w3.org/2000/01/rdf-schema#comment>
                "The WGS84 altitude of a SpatialThing (decimal meters above the local reference ellipsoid)."@en ;
        <http://www.w3.org/2000/01/rdf-schema#domain>
                <https://w3id.org/i40/rami#Machine> ;
        <http://www.w3.org/2000/01/rdf-schema#label>
                "lat"@en ;
        <http://www.w3.org/2000/01/rdf-schema#range>
                <http://www.w3.org/2001/XMLSchema#decimal> .

<https://w3id.org/i40/rami#recordedTime>
        a       <http://www.w3.org/2002/07/owl#DatatypeProperty> ;
        <http://www.w3.org/2000/01/rdf-schema#comment>
                "Recorded Time for a Machine"@en ;
        <http://www.w3.org/2000/01/rdf-schema#domain>
                <https://w3id.org/i40/rami#Machine> ;
        <http://www.w3.org/2000/01/rdf-schema#range>
                <http://www.w3.org/2001/XMLSchema#dateTime> ;
        <http://www.w3.org/2004/02/skos/core#prefLabel>
                "recorded Time"@en .

<https://w3id.org/i40/rami#hasAdminShellId>
        a       <http://www.w3.org/2002/07/owl#FunctionalProperty> , <http://www.w3.org/2002/07/owl#DatatypeProperty> ;
        <http://www.w3.org/2000/01/rdf-schema#domain>
                <https://w3id.org/i40/rami#AdminShell> ;
        <http://www.w3.org/2000/01/rdf-schema#range>
                <http://www.w3.org/2001/XMLSchema#string> ;
        <http://www.w3.org/2000/01/rdf-schema#subPropertyOf>
                dcterms:identifier ;
        <http://www.w3.org/2004/02/skos/core#definition>
                "Unique Identification of the Administration Shell"@en ;
        <http://www.w3.org/2004/02/skos/core#prefLabel>
                "has AdminShell Id"@en .

<https://w3id.org/i40/rami#hasSubmodel>
        a       <http://www.w3.org/2002/07/owl#ObjectProperty> ;
        <http://www.w3.org/2000/01/rdf-schema#comment>
                "Points to the Admin Shell to the Submodels that describe the Admin Shell of a given Asset"@en ;
        <http://www.w3.org/2000/01/rdf-schema#domain>
                <https://w3id.org/i40/rami#AdminShell> ;
        <http://www.w3.org/2000/01/rdf-schema#label>
                "has Submodel"@en ;
        <http://www.w3.org/2000/01/rdf-schema#range>
                <https://w3id.org/i40/rami#Submodel> .

<https://w3id.org/i40/rami#EnergyEfficiency1>
        a       <http://www.w3.org/2002/07/owl#NamedIndividual> , <https://w3id.org/i40/rami#EnergyEfficiency> ;
        <http://www.w3.org/2000/01/rdf-schema#label>
                "Energy Efficiency 1 Submodel"@en ;
        <http://www.w3.org/2004/02/skos/core#definition>
                "Integrated electrical consumption over time."@en ;
        <http://www.w3.org/2004/02/skos/core#prefLabel>
                "Electrical consumption cumulative energy"@en ;
        <https://w3id.org/i40/rami#energyEfficiencyValue>
                <https://w3id.org/i40/rami#MeasureEnergyEfficiency1> ;
        <https://w3id.org/i40/rami#hasSemanticExpression>
                <https://w3id.org/i40/rami#Measurement> ;
        <https://w3id.org/i40/rami#hasView>
                <https://w3id.org/i40/rami#Performance> ;
        <https://w3id.org/i40/rami#subModelID>
                "AAB012" .

<https://w3id.org/i40/rami#BusinessView>
        a       <http://www.w3.org/2002/07/owl#NamedIndividual> , <https://w3id.org/i40/rami#View> ;
        <http://www.w3.org/2000/01/rdf-schema#label>
                "Business"@en , "Allows judging on the business suitability and performance of an asset.\nExamples: Manufacturer name, prices, terms of delivery, order codes.”"@en .

<https://w3id.org/i40/rami#Location>
        a       <http://www.w3.org/2002/07/owl#NamedIndividual> , <https://w3id.org/i40/rami#View> ;
        <http://www.w3.org/2000/01/rdf-schema#comment>
                "Describes the capabilities of the asset regarding environmental conditions and positions of the asset.\nDescribes the relationships capabilities of the asset or its parts or inputs and outputs with the linked assets.\nExamples: Degree of protection, working temperature, EMC characteristics, rated voltage, rated ultimate  \nshort-circuit breaking capacity."@en ;
        <http://www.w3.org/2000/01/rdf-schema#label>
                "Location"@en .

<https://w3id.org/i40/rami#Performance>
        a       <http://www.w3.org/2002/07/owl#NamedIndividual> , <https://w3id.org/i40/rami#View> ;
        <http://www.w3.org/2000/01/rdf-schema#comment>
                "Describes performance and behavioural characteristics. Examples: To allow a performance assessment and virtual commissioning of an overall system. Example: instantaneous short-circuit current setting"@en ;
        <http://www.w3.org/2000/01/rdf-schema#label>
                "Performance"@en .

<https://w3id.org/i40/rami#description>
        a       <http://www.w3.org/2002/07/owl#DatatypeProperty> ;
        <http://www.w3.org/2000/01/rdf-schema#domain>
                <https://w3id.org/i40/rami#Asset> ;
        <http://www.w3.org/2000/01/rdf-schema#range>
                <http://www.w3.org/2001/XMLSchema#string> ;
        <http://www.w3.org/2004/02/skos/core#definition>
                "Description of the Object/Entity"@en ;
        <http://www.w3.org/2004/02/skos/core#prefLabel>
                "has Description"@en .

<https://w3id.org/i40/rami#Measurement>
        a       <http://www.w3.org/2002/07/owl#NamedIndividual> , <https://w3id.org/i40/rami#ExpressionSemantic> ;
        <http://www.w3.org/2000/01/rdf-schema#comment>
                "If a measured or actual value is provided"@en ;
        <http://www.w3.org/2000/01/rdf-schema#label>
                "Measurement"@en .

<https://w3id.org/i40/rami#hasView>
        a       <http://www.w3.org/2002/07/owl#ObjectProperty> ;
        <http://www.w3.org/2000/01/rdf-schema#comment>
                "Points to the differents views associated to the Administration Shell via the Submodels."@en ;
        <http://www.w3.org/2000/01/rdf-schema#domain>
                <https://w3id.org/i40/rami#Submodel> ;
        <http://www.w3.org/2000/01/rdf-schema#label>
                "has View"@en ;
        <http://www.w3.org/2000/01/rdf-schema#range>
                <https://w3id.org/i40/rami#View> .

<https://w3id.org/i40/rami#logs>
        a       <http://www.w3.org/2002/07/owl#DatatypeProperty> ;
        <http://www.w3.org/2000/01/rdf-schema#range>
                <http://www.w3.org/2001/XMLSchema#string> ;
        <http://www.w3.org/2004/02/skos/core#prefLabel>
                "logs"@en .

<http://purl.oclc.org/NET/ssnx/ssn#SensorOutput>
        a       <http://www.w3.org/2002/07/owl#Class> ;
        <http://www.w3.org/2002/07/owl#equivalentClass>
                <https://w3id.org/i40/rami#SensorMeasurementData> .

<http://purl.org/dc/elements/1.1/contributor>
        a       <http://www.w3.org/2002/07/owl#AnnotationProperty> .

<https://w3id.org/i40/rami#hasRAMILifeCycleLayer>
        a       <http://www.w3.org/2002/07/owl#ObjectProperty> ;
        <http://www.w3.org/2004/02/skos/core#definition>
                "Connects the concepts with the correspondent layer in the RAMI Hierarchy Levels"@en ;
        <http://www.w3.org/2004/02/skos/core#prefLabel>
                "has RAMI Life Cycle Layer" .

<https://w3id.org/i40/rami#receivedAtTime>
        a       <http://www.w3.org/2002/07/owl#DatatypeProperty> ;
        <http://www.w3.org/2000/01/rdf-schema#domain>
                <https://w3id.org/i40/rami#AdminShell> ;
        <http://www.w3.org/2000/01/rdf-schema#range>
                <http://www.w3.org/2001/XMLSchema#dateTime> ;
        <http://www.w3.org/2004/02/skos/core#definition>
                "received Time of an Asset"@en ;
        <http://www.w3.org/2004/02/skos/core#prefLabel>
                "received At Time"@en .

<https://w3id.org/i40/rami#hasEnergyValue>
        a       <http://www.w3.org/2002/07/owl#DatatypeProperty> ;
        <http://www.w3.org/2000/01/rdf-schema#domain>
                <https://w3id.org/i40/rami#CumulativeEnergyConsumption> ;
        <http://www.w3.org/2000/01/rdf-schema#range>
                <http://www.w3.org/2001/XMLSchema#float> ;
        <http://www.w3.org/2004/02/skos/core#prefLabel>
                "has Energy Value"@en .

<http://purl.org/dc/elements/1.1/date>
        a       <http://www.w3.org/2002/07/owl#AnnotationProperty> .

<http://purl.org/dc/elements/1.1/rights>
        a       <http://www.w3.org/2002/07/owl#AnnotationProperty> .

<https://w3id.org/i40/rami#hasDatatype>
        a       <http://www.w3.org/2002/07/owl#ObjectProperty> ;
        <http://www.w3.org/2000/01/rdf-schema#comment>
                "Points to the datatypes of the Submodels"@en ;
        <http://www.w3.org/2000/01/rdf-schema#domain>
                <https://w3id.org/i40/rami#Submodel> ;
        <http://www.w3.org/2000/01/rdf-schema#label>
                "has Datatype"@en .

dcterms:description  a  <http://www.w3.org/2002/07/owl#AnnotationProperty> .

<https://w3id.org/i40/rami#ComponentManager>
        a       <http://www.w3.org/2002/07/owl#Class> ;
        <http://www.w3.org/2000/01/rdf-schema#label>
                "Component Manager"@en .

<http://xmlns.com/foaf/spec/Image>
        a       <http://www.w3.org/2002/07/owl#Class> .

<https://w3id.org/i40/rami#ITLayerDimension>
        a       <http://www.w3.org/2002/07/owl#Class> ;
        <http://www.w3.org/2000/01/rdf-schema#label>
                "RAMI IT Layer Dimension"@en ;
        <http://www.w3.org/2000/01/rdf-schema#subClassOf>
                <https://w3id.org/i40/rami#Dimension> ;
        <http://www.w3.org/2002/07/owl#equivalentClass>
                [ a       <http://www.w3.org/2002/07/owl#Class> ;
                  <http://www.w3.org/2002/07/owl#oneOf>
                          ( <https://w3id.org/i40/rami#Asset> <https://w3id.org/i40/rami#Business> <https://w3id.org/i40/rami#Communication> <https://w3id.org/i40/rami#Functional> <https://w3id.org/i40/rami#Information> <https://w3id.org/i40/rami#Integration> )
                ] .

<https://w3id.org/i40/rami#Confirmation>
        a       <http://www.w3.org/2002/07/owl#NamedIndividual> , <https://w3id.org/i40/rami#ExpressionSemantic> ;
        <http://www.w3.org/2000/01/rdf-schema#comment>
                "For responses to requests that describe the capability of an asset."@en ;
        <http://www.w3.org/2000/01/rdf-schema#label>
                "Confirmation"@en .

<https://w3id.org/i40/rami#hasValue>
        a       <http://www.w3.org/2002/07/owl#ObjectProperty> ;
        <http://www.w3.org/2000/01/rdf-schema#comment>
                "Points to the current value that can be specified through an instanced submodel (for \ninstance in station 2) or through the asset."@en ;
        <http://www.w3.org/2000/01/rdf-schema#domain>
                <https://w3id.org/i40/rami#Submodel> ;
        <http://www.w3.org/2000/01/rdf-schema#label>
                "has Value"@en ;
        <http://www.w3.org/2000/01/rdf-schema#range>
                <https://w3id.org/i40/rami#Value> .

<https://w3id.org/i40/rami#publishedURL>
        a       <http://www.w3.org/2002/07/owl#DatatypeProperty> .

<http://purl.org/dc/elements/1.1/title>
        a       <http://www.w3.org/2002/07/owl#AnnotationProperty> .

<https://w3id.org/i40/rami#releaseDate>
        a       <http://www.w3.org/2002/07/owl#DatatypeProperty> ;
        <http://www.w3.org/2000/01/rdf-schema#range>
                <http://www.w3.org/2001/XMLSchema#date> ;
        <http://www.w3.org/2004/02/skos/core#definition>
                "Release Date of the Standard"@en ;
        <http://www.w3.org/2004/02/skos/core#prefLabel>
                "Release Date"@en .

<http://www.w3.org/2001/XMLSchema#date>
        a       <http://www.w3.org/2000/01/rdf-schema#Datatype> .

<https://w3id.org/i40/rami#Platform1>
        a       <http://www.w3.org/2002/07/owl#NamedIndividual> .

<https://w3id.org/i40/rami#hasRAMIHierarchyLevel>
        a       <http://www.w3.org/2002/07/owl#ObjectProperty> ;
        <http://www.w3.org/2000/01/rdf-schema#range>
                <https://w3id.org/i40/rami#HierarchyLevelDimension> ;
        <http://www.w3.org/2004/02/skos/core#definition>
                "Connects the concepts with the correspondent layer in the RAMI Hierarchy Levels"@en ;
        <http://www.w3.org/2004/02/skos/core#prefLabel>
                "has RAMI Hierarchy Level"@en .

<https://w3id.org/i40/rami#Information>
        a       <http://www.w3.org/2002/07/owl#NamedIndividual> .

<http://www.w3.org/2003/01/geo/wgs84_pos#long>
        a       <http://www.w3.org/2002/07/owl#DatatypeProperty> ;
        <http://www.w3.org/2000/01/rdf-schema#comment>
                "The WGS84 longitude of a SpatialThing (decimal degrees)."@en ;
        <http://www.w3.org/2000/01/rdf-schema#domain>
                <https://w3id.org/i40/rami#Machine> ;
        <http://www.w3.org/2000/01/rdf-schema#label>
                "long"@en ;
        <http://www.w3.org/2000/01/rdf-schema#range>
                <http://www.w3.org/2001/XMLSchema#decimal> .

<http://purl.org/dc/elements/1.1/type>
        a       <http://www.w3.org/2002/07/owl#AnnotationProperty> .

<https://w3id.org/i40/rami#Asset2>
        a       <http://www.w3.org/2002/07/owl#NamedIndividual> , <https://w3id.org/i40/rami#Asset> ;
        <http://www.w3.org/2000/01/rdf-schema#label>
                "Asset 2"@en ;
        <https://w3id.org/i40/rami#hasAssetId>
                "AS712" .

<https://w3id.org/i40/rami#hasReference>
        a       <http://www.w3.org/2002/07/owl#ObjectProperty> ;
        <http://www.w3.org/2000/01/rdf-schema#domain>
                <https://w3id.org/i40/rami#Submodel> ;
        <http://www.w3.org/2000/01/rdf-schema#label>
                "has Reference"@en .

<https://w3id.org/i40/rami#hasComponentManager>
        a       <http://www.w3.org/2002/07/owl#ObjectProperty> ;
        <http://www.w3.org/2000/01/rdf-schema#domain>
                <https://w3id.org/i40/rami#AdminShell> ;
        <http://www.w3.org/2000/01/rdf-schema#label>
                "has Component Manager"@en ;
        <http://www.w3.org/2000/01/rdf-schema#range>
                <https://w3id.org/i40/rami#ComponentManager> .

<http://xmlns.com/foaf/spec/image>
        a       <http://www.w3.org/2002/07/owl#DatatypeProperty> , <http://www.w3.org/2002/07/owl#AnnotationProperty> ;
        <http://www.w3.org/2000/01/rdf-schema#comment>
                "Image of the Asset reused from the FOAF ontology."@en ;
        <http://www.w3.org/2000/01/rdf-schema#domain>
                <https://w3id.org/i40/rami#Asset> ;
        <http://www.w3.org/2000/01/rdf-schema#label>
                "image"@en ;
        <http://www.w3.org/2000/01/rdf-schema#range>
                <http://www.w3.org/2001/XMLSchema#anyURI> .

<https://w3id.org/i40/rami#EnergyEfficiency2>
        a       <http://www.w3.org/2002/07/owl#NamedIndividual> , <https://w3id.org/i40/rami#EnergyEfficiency> ;
        <http://www.w3.org/2000/01/rdf-schema#label>
                "Energy Efficiency 2 Submodel"@en ;
        <https://w3id.org/i40/rami#energyEfficiencyValue>
                <https://w3id.org/i40/rami#MeasureEnergyEfficiency2> ;
        <https://w3id.org/i40/rami#subModelID>
                "AAB013" .

<https://w3id.org/i40/rami#inventoryNumber>
        a       <http://www.w3.org/2002/07/owl#FunctionalProperty> , <http://www.w3.org/2002/07/owl#DatatypeProperty> ;
        <http://www.w3.org/2000/01/rdf-schema#domain>
                <https://w3id.org/i40/rami#Asset> ;
        <http://www.w3.org/2000/01/rdf-schema#range>
                <http://www.w3.org/2001/XMLSchema#string> ;
        <http://www.w3.org/2004/02/skos/core#definition>
                "Inventory number of the Entity/Object according to the identification nomenclature"@en ;
        <http://www.w3.org/2004/02/skos/core#prefLabel>
                "Inventory Number"@en .

<https://w3id.org/i40/rami#TransportInterface>
        a       <http://www.w3.org/2002/07/owl#Class> ;
        <http://www.w3.org/2000/01/rdf-schema#subClassOf>
                <https://w3id.org/i40/rami#Submodel> .

[ a       <http://www.w3.org/2002/07/owl#AllDisjointClasses> ;
  <http://www.w3.org/2002/07/owl#members>
          ( <https://w3id.org/i40/rami#HierarchyLevelDimension> <https://w3id.org/i40/rami#ITLayerDimension> <https://w3id.org/i40/rami#LifeCycleDimension> )
] .
